src/code/kubernetes_model/apimodel.v
@@ -33,6 +33,7 @@ Require Export New.code.k8s_io.kubernetes.pkg.registry.apps.replicaset.
 Require Export New.code.k8s_io.kubernetes.pkg.registry.apps.statefulset.
 Require Export New.code.k8s_io.kubernetes.pkg.registry.core.persistentvolumeclaim.
 Require Export New.code.k8s_io.kubernetes.pkg.registry.core.pod.
+Require Export New.code.k8s_io.kubernetes.pkg.registry.core.serviceaccount.
 Require Export New.code.k8s_io.kubernetes.pkg.apis.apps.install.
 Module api_apps_v1 := code.k8s_io.api.apps.v1.v1.
 Module api_core_v1 := code.k8s_io.api.core.v1.v1.
@@ -143,7 +144,7 @@ Definition preconditionUIDMismatch {ext : ffi_syntax} {go_gctx : GoGlobalContext
 
 Definition setPreconditionResourceVersion {ext : ffi_syntax} {go_gctx : GoGlobalContext} : go_string := "kubernetes_model/apimodel.setPreconditionResourceVersion"%go.
 
-(* go: api_model.go:81:6 *)
+(* go: api_model.go:82:6 *)
 Definition NewStateⁱᵐᵖˡ {ext : ffi_syntax} {go_gctx : GoGlobalContext} : val :=
   λ: <>,
     exception_do (return: (GoAlloc State (let: "$v0" := ((FuncResolve go.make1 [go.MapType KKey (go.InterfaceType [])] #()) #()) in
@@ -161,7 +162,7 @@ Definition NewStateⁱᵐᵖˡ {ext : ffi_syntax} {go_gctx : GoGlobalContext} : 
 
       ])) "$v2"); KeyedElement (Some (KeyField "resourceVersionCounter"%go)) (ElementExpression go.int64 "$v3"); KeyedElement (Some (KeyField "mu"%go)) (ElementExpression (go.PointerType sync.Mutex) "$v4")])))).
 
-(* go: api_model.go:91:6 *)
+(* go: api_model.go:92:6 *)
 Definition deepCopyⁱᵐᵖˡ {ext : ffi_syntax} {go_gctx : GoGlobalContext} : val :=
   λ: "obj",
     exception_do (let: "obj" := (GoAlloc (go.InterfaceType []) "obj") in
@@ -178,31 +179,43 @@ Definition deepCopyⁱᵐᵖˡ {ext : ffi_syntax} {go_gctx : GoGlobalContext} : 
         let: "o" := (GoAlloc (go.PointerType api_core_v1.PersistentVolumeClaim) "$x") in
         return: (Convert (go.PointerType api_core_v1.PersistentVolumeClaim) (go.InterfaceType []) ((MethodResolve (go.PointerType api_core_v1.PersistentVolumeClaim) "DeepCopy"%go (![go.PointerType api_core_v1.PersistentVolumeClaim] "o")) #()))
       else
-        let: ("$x", "$ok") := (TypeAssert2 (go.PointerType api_apps_v1.ReplicaSet) "$y") in
+        let: ("$x", "$ok") := (TypeAssert2 (go.PointerType api_core_v1.Namespace) "$y") in
         (if: "$ok"
         then
-          let: "o" := (GoAlloc (go.PointerType api_apps_v1.ReplicaSet) "$x") in
-          return: (Convert (go.PointerType api_apps_v1.ReplicaSet) (go.InterfaceType []) ((MethodResolve (go.PointerType api_apps_v1.ReplicaSet) "DeepCopy"%go (![go.PointerType api_apps_v1.ReplicaSet] "o")) #()))
+          let: "o" := (GoAlloc (go.PointerType api_core_v1.Namespace) "$x") in
+          return: (Convert (go.PointerType api_core_v1.Namespace) (go.InterfaceType []) ((MethodResolve (go.PointerType api_core_v1.Namespace) "DeepCopy"%go (![go.PointerType api_core_v1.Namespace] "o")) #()))
         else
-          let: ("$x", "$ok") := (TypeAssert2 (go.PointerType api_apps_v1.StatefulSet) "$y") in
+          let: ("$x", "$ok") := (TypeAssert2 (go.PointerType api_core_v1.ServiceAccount) "$y") in
           (if: "$ok"
           then
-            let: "o" := (GoAlloc (go.PointerType api_apps_v1.StatefulSet) "$x") in
-            return: (Convert (go.PointerType api_apps_v1.StatefulSet) (go.InterfaceType []) ((MethodResolve (go.PointerType api_apps_v1.StatefulSet) "DeepCopy"%go (![go.PointerType api_apps_v1.StatefulSet] "o")) #()))
+            let: "o" := (GoAlloc (go.PointerType api_core_v1.ServiceAccount) "$x") in
+            return: (Convert (go.PointerType api_core_v1.ServiceAccount) (go.InterfaceType []) ((MethodResolve (go.PointerType api_core_v1.ServiceAccount) "DeepCopy"%go (![go.PointerType api_core_v1.ServiceAccount] "o")) #()))
           else
-            let: ("$x", "$ok") := (TypeAssert2 (go.PointerType api_apps_v1.Deployment) "$y") in
+            let: ("$x", "$ok") := (TypeAssert2 (go.PointerType api_apps_v1.ReplicaSet) "$y") in
             (if: "$ok"
             then
-              let: "o" := (GoAlloc (go.PointerType api_apps_v1.Deployment) "$x") in
-              return: (Convert (go.PointerType api_apps_v1.Deployment) (go.InterfaceType []) ((MethodResolve (go.PointerType api_apps_v1.Deployment) "DeepCopy"%go (![go.PointerType api_apps_v1.Deployment] "o")) #()))
+              let: "o" := (GoAlloc (go.PointerType api_apps_v1.ReplicaSet) "$x") in
+              return: (Convert (go.PointerType api_apps_v1.ReplicaSet) (go.InterfaceType []) ((MethodResolve (go.PointerType api_apps_v1.ReplicaSet) "DeepCopy"%go (![go.PointerType api_apps_v1.ReplicaSet] "o")) #()))
             else
-              do:  (let: "$a0" := (Convert go.string (go.InterfaceType []) (let: "$a0" := #"copyObject: unsupported type %T"%go in
-              let: "$a1" := ((let: "$sl0" := (![go.InterfaceType []] "obj") in
-              CompositeLiteral (go.SliceType go.any) (LiteralValue [KeyedElement None (ElementExpression go.any "$sl0")]))) in
-              (FuncResolve fmt.Sprintf [] #()) "$a0" "$a1")) in
-              (FuncResolve go.panic [] #()) "$a0"))))))).
+              let: ("$x", "$ok") := (TypeAssert2 (go.PointerType api_apps_v1.StatefulSet) "$y") in
+              (if: "$ok"
+              then
+                let: "o" := (GoAlloc (go.PointerType api_apps_v1.StatefulSet) "$x") in
+                return: (Convert (go.PointerType api_apps_v1.StatefulSet) (go.InterfaceType []) ((MethodResolve (go.PointerType api_apps_v1.StatefulSet) "DeepCopy"%go (![go.PointerType api_apps_v1.StatefulSet] "o")) #()))
+              else
+                let: ("$x", "$ok") := (TypeAssert2 (go.PointerType api_apps_v1.Deployment) "$y") in
+                (if: "$ok"
+                then
+                  let: "o" := (GoAlloc (go.PointerType api_apps_v1.Deployment) "$x") in
+                  return: (Convert (go.PointerType api_apps_v1.Deployment) (go.InterfaceType []) ((MethodResolve (go.PointerType api_apps_v1.Deployment) "DeepCopy"%go (![go.PointerType api_apps_v1.Deployment] "o")) #()))
+                else
+                  do:  (let: "$a0" := (Convert go.string (go.InterfaceType []) (let: "$a0" := #"copyObject: unsupported type %T"%go in
+                  let: "$a1" := ((let: "$sl0" := (![go.InterfaceType []] "obj") in
+                  CompositeLiteral (go.SliceType go.any) (LiteralValue [KeyedElement None (ElementExpression go.any "$sl0")]))) in
+                  (FuncResolve fmt.Sprintf [] #()) "$a0" "$a1")) in
+                  (FuncResolve go.panic [] #()) "$a0"))))))))).
 
-(* go: api_model.go:108:17 *)
+(* go: api_model.go:113:17 *)
 Definition State__objListLockedⁱᵐᵖˡ {ext : ffi_syntax} {go_gctx : GoGlobalContext} : val :=
   λ: "s" "kind" "namespace",
     exception_do (let: "items" := (GoAlloc (go.SliceType (go.InterfaceType [])) (GoZeroVal (go.SliceType (go.InterfaceType [])) #())) in
@@ -229,7 +242,7 @@ Definition State__objListLockedⁱᵐᵖˡ {ext : ffi_syntax} {go_gctx : GoGloba
       else do:  #())));;;
     return: (![go.SliceType (go.InterfaceType [])] "items")).
 
-(* go: api_model.go:119:17 *)
+(* go: api_model.go:124:17 *)
 Definition State__objListⁱᵐᵖˡ {ext : ffi_syntax} {go_gctx : GoGlobalContext} : val :=
   λ: "s" "kind" "namespace",
     with_defer: (let: "items" := (GoAlloc (go.SliceType (go.InterfaceType [])) (GoZeroVal (go.SliceType (go.InterfaceType [])) #())) in
@@ -247,7 +260,7 @@ Definition State__objListⁱᵐᵖˡ {ext : ffi_syntax} {go_gctx : GoGlobalConte
      let: "$a1" := (![go.string] "namespace") in
      (MethodResolve (go.PointerType State) "objListLocked"%go (![go.PointerType State] "s")) "$a0" "$a1")).
 
-(* go: api_model.go:126:6 *)
+(* go: api_model.go:131:6 *)
 Definition filterByLabelSelectorⁱᵐᵖˡ {ext : ffi_syntax} {go_gctx : GoGlobalContext} : val :=
   λ: "items" "selector",
     exception_do (let: "selector" := (GoAlloc labels.Selector "selector") in
@@ -280,7 +293,7 @@ Definition filterByLabelSelectorⁱᵐᵖˡ {ext : ffi_syntax} {go_gctx : GoGlob
       else do:  #())));;;
     return: (![go.SliceType (go.InterfaceType [])] "filtered_items", Convert go.untyped_nil go.error UntypedNil)).
 
-(* go: api_model.go:140:17 *)
+(* go: api_model.go:145:17 *)
 Definition State__objListBySelectorⁱᵐᵖˡ {ext : ffi_syntax} {go_gctx : GoGlobalContext} : val :=
   λ: "s" "kind" "namespace" "selector",
     exception_do (let: "s" := (GoAlloc (go.PointerType State) "s") in
@@ -294,7 +307,7 @@ Definition State__objListBySelectorⁱᵐᵖˡ {ext : ffi_syntax} {go_gctx : GoG
     (FuncResolve filterByLabelSelector [] #()) "$a0" "$a1")) in
     return: ("$ret0", "$ret1")).
 
-(* go: api_model.go:144:6 *)
+(* go: api_model.go:149:6 *)
 Definition index_ofⁱᵐᵖˡ {ext : ffi_syntax} {go_gctx : GoGlobalContext} : val :=
   λ: "indexName" "obj",
     exception_do (let: "obj" := (GoAlloc (go.InterfaceType []) "obj") in
@@ -324,7 +337,7 @@ Definition index_ofⁱᵐᵖˡ {ext : ffi_syntax} {go_gctx : GoGlobalContext} : 
 
 (* Returned value must be treated as read-only.
 
-   go: api_model.go:159:17 *)
+   go: api_model.go:164:17 *)
 Definition State__Indexⁱᵐᵖˡ {ext : ffi_syntax} {go_gctx : GoGlobalContext} : val :=
   λ: "s" "kind" "indexName" "obj",
     with_defer: (let: "s" := (GoAlloc (go.PointerType State) "s") in
@@ -425,7 +438,7 @@ Definition State__Indexⁱᵐᵖˡ {ext : ffi_syntax} {go_gctx : GoGlobalContext
 
 (* Returned value must be treated as read-only.
 
-   go: api_model.go:194:17 *)
+   go: api_model.go:199:17 *)
 Definition State__ByIndexⁱᵐᵖˡ {ext : ffi_syntax} {go_gctx : GoGlobalContext} : val :=
   λ: "s" "kind" "indexName" "indexedValue",
     with_defer: (let: "s" := (GoAlloc (go.PointerType State) "s") in
@@ -478,7 +491,7 @@ Definition State__ByIndexⁱᵐᵖˡ {ext : ffi_syntax} {go_gctx : GoGlobalConte
         else do:  #())))));;;
     return: (![go.SliceType (go.InterfaceType [])] "items", Convert go.untyped_nil go.error UntypedNil)).
 
-(* go: api_model.go:215:17 *)
+(* go: api_model.go:220:17 *)
 Definition State__getⁱᵐᵖˡ {ext : ffi_syntax} {go_gctx : GoGlobalContext} : val :=
   λ: "s" "key",
     with_defer: (let: "s" := (GoAlloc (go.PointerType State) "s") in
@@ -507,7 +520,7 @@ Definition State__getⁱᵐᵖˡ {ext : ffi_syntax} {go_gctx : GoGlobalContext} 
        let: "$a1" := (![go.string] (StructFieldRef KKey "Name"%go "key")) in
        (FuncResolve errors.NewNotFound [] #()) "$a0" "$a1")))).
 
-(* go: api_model.go:228:6 *)
+(* go: api_model.go:233:6 *)
 Definition randomSuffixⁱᵐᵖˡ {ext : ffi_syntax} {go_gctx : GoGlobalContext} : val :=
   λ: "n",
     exception_do (let: "n" := (GoAlloc go.int "n") in
@@ -532,7 +545,7 @@ Definition randomSuffixⁱᵐᵖˡ {ext : ffi_syntax} {go_gctx : GoGlobalContext
       do:  ((IndexRef (go.SliceType go.byte) (![go.SliceType go.byte] "b", ![go.int] "i")) <-[go.byte] "$r0")));;;
     return: (Convert (go.SliceType go.byte) go.string (![go.SliceType go.byte] "b"))).
 
-(* go: api_model.go:238:17 *)
+(* go: api_model.go:243:17 *)
 Definition State__generateNewNameⁱᵐᵖˡ {ext : ffi_syntax} {go_gctx : GoGlobalContext} : val :=
   λ: "s" "kind" "namespace" "generateName",
     exception_do (let: "s" := (GoAlloc (go.PointerType State) "s") in
@@ -560,7 +573,7 @@ Definition State__generateNewNameⁱᵐᵖˡ {ext : ffi_syntax} {go_gctx : GoGlo
       then return: (![go.string] "name")
       else do:  #())))).
 
-(* go: api_model.go:252:17 *)
+(* go: api_model.go:257:17 *)
 Definition State__generateNewUIDAndUpdateⁱᵐᵖˡ {ext : ffi_syntax} {go_gctx : GoGlobalContext} : val :=
   λ: "s" <>,
     exception_do (let: "s" := (GoAlloc (go.PointerType State) "s") in
@@ -589,7 +602,7 @@ Definition State__generateNewUIDAndUpdateⁱᵐᵖˡ {ext : ffi_syntax} {go_gctx
         return: (![types.UID] "uid")
       else do:  #())))).
 
-(* go: api_model.go:262:17 *)
+(* go: api_model.go:267:17 *)
 Definition State__generateNewRVAndUpdateⁱᵐᵖˡ {ext : ffi_syntax} {go_gctx : GoGlobalContext} : val :=
   λ: "s" <>,
     exception_do (let: "s" := (GoAlloc (go.PointerType State) "s") in
@@ -623,7 +636,7 @@ Definition State__generateNewRVAndUpdateⁱᵐᵖˡ {ext : ffi_syntax} {go_gctx 
 (* validateObjectMeta validates the ObjectMeta fields using generic Kubernetes validation.
    This matches the API server's generic metadata validation that happens in BeforeCreate.
 
-   go: api_model.go:274:6 *)
+   go: api_model.go:279:6 *)
 Definition validateObjectMetaⁱᵐᵖˡ {ext : ffi_syntax} {go_gctx : GoGlobalContext} : val :=
   λ: "metadata" "kind",
     exception_do (let: "kind" := (GoAlloc go.string "kind") in
@@ -656,7 +669,7 @@ Definition validateObjectMetaⁱᵐᵖˡ {ext : ffi_syntax} {go_gctx : GoGlobalC
    node.kubernetes.io/unreachable:NoExecute with 300s toleration seconds.
    Reference: https://github.com/kubernetes/kubernetes/blob/release-1.34/plugin/pkg/admission/defaulttolerationseconds/admission.go
 
-   go: api_model.go:301:6 *)
+   go: api_model.go:306:6 *)
 Definition applyDefaultTolerationSecondsⁱᵐᵖˡ {ext : ffi_syntax} {go_gctx : GoGlobalContext} : val :=
   λ: "pod",
     exception_do (let: "pod" := (GoAlloc (go.PointerType core.Pod) "pod") in
@@ -734,7 +747,7 @@ Definition applyDefaultTolerationSecondsⁱᵐᵖˡ {ext : ffi_syntax} {go_gctx 
    - If PriorityClassName is specified, we cannot look it up (not implemented), so we skip
    Reference: https://github.com/kubernetes/kubernetes/blob/release-1.34/plugin/pkg/admission/priority/admission.go
 
-   go: api_model.go:355:6 *)
+   go: api_model.go:360:6 *)
 Definition applyPriorityAdmissionⁱᵐᵖˡ {ext : ffi_syntax} {go_gctx : GoGlobalContext} : val :=
   λ: "pod",
     exception_do (let: "pod" := (GoAlloc (go.PointerType core.Pod) "pod") in
@@ -757,7 +770,7 @@ Definition applyPriorityAdmissionⁱᵐᵖˡ {ext : ffi_syntax} {go_gctx : GoGlo
 (* convertVersionedToLegacy converts supported external/versioned API objects
    to their internal Kubernetes representations.
 
-   go: api_model.go:376:6 *)
+   go: api_model.go:381:6 *)
 Definition convertVersionedToLegacyⁱᵐᵖˡ {ext : ffi_syntax} {go_gctx : GoGlobalContext} : val :=
   λ: "obj",
     exception_do (let: "obj" := (GoAlloc (go.InterfaceType []) "obj") in
@@ -808,85 +821,108 @@ Definition convertVersionedToLegacyⁱᵐᵖˡ {ext : ffi_syntax} {go_gctx : GoG
         else do:  #()));;;
         return: (Convert (go.PointerType core.PersistentVolumeClaim) (go.InterfaceType []) (![go.PointerType core.PersistentVolumeClaim] "internalPVC"), Convert go.untyped_nil go.error UntypedNil)
       else
-        let: ("$x", "$ok") := (TypeAssert2 (go.PointerType api_apps_v1.ReplicaSet) "$y") in
+        let: ("$x", "$ok") := (TypeAssert2 (go.PointerType api_core_v1.ServiceAccount) "$y") in
         (if: "$ok"
         then
-          let: "typed" := (GoAlloc (go.PointerType api_apps_v1.ReplicaSet) "$x") in
-          let: "internalRS" := (GoAlloc (go.PointerType apps.ReplicaSet) (GoZeroVal (go.PointerType apps.ReplicaSet) #())) in
-          let: "$r0" := (GoAlloc apps.ReplicaSet (CompositeLiteral apps.ReplicaSet (LiteralValue []))) in
-          do:  ("internalRS" <-[go.PointerType apps.ReplicaSet] "$r0");;;
+          let: "typed" := (GoAlloc (go.PointerType api_core_v1.ServiceAccount) "$x") in
+          let: "internalServiceAccount" := (GoAlloc (go.PointerType core.ServiceAccount) (GoZeroVal (go.PointerType core.ServiceAccount) #())) in
+          let: "$r0" := (GoAlloc core.ServiceAccount (CompositeLiteral core.ServiceAccount (LiteralValue []))) in
+          do:  ("internalServiceAccount" <-[go.PointerType core.ServiceAccount] "$r0");;;
           (let: "err" := (GoAlloc go.error (GoZeroVal go.error #())) in
-          let: "$r0" := (let: "$a0" := (Convert (go.PointerType api_apps_v1.ReplicaSet) (go.InterfaceType []) (![go.PointerType api_apps_v1.ReplicaSet] "typed")) in
-          let: "$a1" := (Convert (go.PointerType apps.ReplicaSet) (go.InterfaceType []) (![go.PointerType apps.ReplicaSet] "internalRS")) in
+          let: "$r0" := (let: "$a0" := (Convert (go.PointerType api_core_v1.ServiceAccount) (go.InterfaceType []) (![go.PointerType api_core_v1.ServiceAccount] "typed")) in
+          let: "$a1" := (Convert (go.PointerType core.ServiceAccount) (go.InterfaceType []) (![go.PointerType core.ServiceAccount] "internalServiceAccount")) in
           let: "$a2" := (Convert go.untyped_nil (go.InterfaceType []) UntypedNil) in
           (MethodResolve (go.PointerType runtime.Scheme) "Convert"%go (![go.PointerType runtime.Scheme] (GlobalVarAddr legacyscheme.Scheme #()))) "$a0" "$a1" "$a2") in
           do:  ("err" <-[go.error] "$r0");;;
           (if: Convert go.untyped_bool go.bool ((![go.error] "err") ≠⟨go.error⟩ (Convert go.untyped_nil go.error UntypedNil))
           then
-            return: (Convert go.untyped_nil (go.InterfaceType []) UntypedNil, Convert (go.PointerType errors.StatusError) go.error (let: "$a0" := (let: "$a0" := #"failed to convert appsv1.ReplicaSet to internal ReplicaSet: %v"%go in
+            return: (Convert go.untyped_nil (go.InterfaceType []) UntypedNil, Convert (go.PointerType errors.StatusError) go.error (let: "$a0" := (let: "$a0" := #"failed to convert v1.ServiceAccount to internal ServiceAccount: %v"%go in
              let: "$a1" := ((let: "$sl0" := (Convert go.error go.any (![go.error] "err")) in
              CompositeLiteral (go.SliceType go.any) (LiteralValue [KeyedElement None (ElementExpression go.any "$sl0")]))) in
              (FuncResolve fmt.Sprintf [] #()) "$a0" "$a1") in
              (FuncResolve errors.NewBadRequest [] #()) "$a0"))
           else do:  #()));;;
-          return: (Convert (go.PointerType apps.ReplicaSet) (go.InterfaceType []) (![go.PointerType apps.ReplicaSet] "internalRS"), Convert go.untyped_nil go.error UntypedNil)
+          return: (Convert (go.PointerType core.ServiceAccount) (go.InterfaceType []) (![go.PointerType core.ServiceAccount] "internalServiceAccount"), Convert go.untyped_nil go.error UntypedNil)
         else
-          let: ("$x", "$ok") := (TypeAssert2 (go.PointerType api_apps_v1.StatefulSet) "$y") in
+          let: ("$x", "$ok") := (TypeAssert2 (go.PointerType api_apps_v1.ReplicaSet) "$y") in
           (if: "$ok"
           then
-            let: "typed" := (GoAlloc (go.PointerType api_apps_v1.StatefulSet) "$x") in
-            let: "internalSTS" := (GoAlloc (go.PointerType apps.StatefulSet) (GoZeroVal (go.PointerType apps.StatefulSet) #())) in
-            let: "$r0" := (GoAlloc apps.StatefulSet (CompositeLiteral apps.StatefulSet (LiteralValue []))) in
-            do:  ("internalSTS" <-[go.PointerType apps.StatefulSet] "$r0");;;
+            let: "typed" := (GoAlloc (go.PointerType api_apps_v1.ReplicaSet) "$x") in
+            let: "internalRS" := (GoAlloc (go.PointerType apps.ReplicaSet) (GoZeroVal (go.PointerType apps.ReplicaSet) #())) in
+            let: "$r0" := (GoAlloc apps.ReplicaSet (CompositeLiteral apps.ReplicaSet (LiteralValue []))) in
+            do:  ("internalRS" <-[go.PointerType apps.ReplicaSet] "$r0");;;
             (let: "err" := (GoAlloc go.error (GoZeroVal go.error #())) in
-            let: "$r0" := (let: "$a0" := (Convert (go.PointerType api_apps_v1.StatefulSet) (go.InterfaceType []) (![go.PointerType api_apps_v1.StatefulSet] "typed")) in
-            let: "$a1" := (Convert (go.PointerType apps.StatefulSet) (go.InterfaceType []) (![go.PointerType apps.StatefulSet] "internalSTS")) in
+            let: "$r0" := (let: "$a0" := (Convert (go.PointerType api_apps_v1.ReplicaSet) (go.InterfaceType []) (![go.PointerType api_apps_v1.ReplicaSet] "typed")) in
+            let: "$a1" := (Convert (go.PointerType apps.ReplicaSet) (go.InterfaceType []) (![go.PointerType apps.ReplicaSet] "internalRS")) in
             let: "$a2" := (Convert go.untyped_nil (go.InterfaceType []) UntypedNil) in
             (MethodResolve (go.PointerType runtime.Scheme) "Convert"%go (![go.PointerType runtime.Scheme] (GlobalVarAddr legacyscheme.Scheme #()))) "$a0" "$a1" "$a2") in
             do:  ("err" <-[go.error] "$r0");;;
             (if: Convert go.untyped_bool go.bool ((![go.error] "err") ≠⟨go.error⟩ (Convert go.untyped_nil go.error UntypedNil))
             then
-              return: (Convert go.untyped_nil (go.InterfaceType []) UntypedNil, Convert (go.PointerType errors.StatusError) go.error (let: "$a0" := (let: "$a0" := #"failed to convert appsv1.StatefulSet to internal StatefulSet: %v"%go in
+              return: (Convert go.untyped_nil (go.InterfaceType []) UntypedNil, Convert (go.PointerType errors.StatusError) go.error (let: "$a0" := (let: "$a0" := #"failed to convert appsv1.ReplicaSet to internal ReplicaSet: %v"%go in
                let: "$a1" := ((let: "$sl0" := (Convert go.error go.any (![go.error] "err")) in
                CompositeLiteral (go.SliceType go.any) (LiteralValue [KeyedElement None (ElementExpression go.any "$sl0")]))) in
                (FuncResolve fmt.Sprintf [] #()) "$a0" "$a1") in
                (FuncResolve errors.NewBadRequest [] #()) "$a0"))
             else do:  #()));;;
-            return: (Convert (go.PointerType apps.StatefulSet) (go.InterfaceType []) (![go.PointerType apps.StatefulSet] "internalSTS"), Convert go.untyped_nil go.error UntypedNil)
+            return: (Convert (go.PointerType apps.ReplicaSet) (go.InterfaceType []) (![go.PointerType apps.ReplicaSet] "internalRS"), Convert go.untyped_nil go.error UntypedNil)
           else
-            let: ("$x", "$ok") := (TypeAssert2 (go.PointerType api_apps_v1.Deployment) "$y") in
+            let: ("$x", "$ok") := (TypeAssert2 (go.PointerType api_apps_v1.StatefulSet) "$y") in
             (if: "$ok"
             then
-              let: "typed" := (GoAlloc (go.PointerType api_apps_v1.Deployment) "$x") in
-              let: "internalDeployment" := (GoAlloc (go.PointerType apps.Deployment) (GoZeroVal (go.PointerType apps.Deployment) #())) in
-              let: "$r0" := (GoAlloc apps.Deployment (CompositeLiteral apps.Deployment (LiteralValue []))) in
-              do:  ("internalDeployment" <-[go.PointerType apps.Deployment] "$r0");;;
+              let: "typed" := (GoAlloc (go.PointerType api_apps_v1.StatefulSet) "$x") in
+              let: "internalSTS" := (GoAlloc (go.PointerType apps.StatefulSet) (GoZeroVal (go.PointerType apps.StatefulSet) #())) in
+              let: "$r0" := (GoAlloc apps.StatefulSet (CompositeLiteral apps.StatefulSet (LiteralValue []))) in
+              do:  ("internalSTS" <-[go.PointerType apps.StatefulSet] "$r0");;;
               (let: "err" := (GoAlloc go.error (GoZeroVal go.error #())) in
-              let: "$r0" := (let: "$a0" := (Convert (go.PointerType api_apps_v1.Deployment) (go.InterfaceType []) (![go.PointerType api_apps_v1.Deployment] "typed")) in
-              let: "$a1" := (Convert (go.PointerType apps.Deployment) (go.InterfaceType []) (![go.PointerType apps.Deployment] "internalDeployment")) in
+              let: "$r0" := (let: "$a0" := (Convert (go.PointerType api_apps_v1.StatefulSet) (go.InterfaceType []) (![go.PointerType api_apps_v1.StatefulSet] "typed")) in
+              let: "$a1" := (Convert (go.PointerType apps.StatefulSet) (go.InterfaceType []) (![go.PointerType apps.StatefulSet] "internalSTS")) in
               let: "$a2" := (Convert go.untyped_nil (go.InterfaceType []) UntypedNil) in
               (MethodResolve (go.PointerType runtime.Scheme) "Convert"%go (![go.PointerType runtime.Scheme] (GlobalVarAddr legacyscheme.Scheme #()))) "$a0" "$a1" "$a2") in
               do:  ("err" <-[go.error] "$r0");;;
               (if: Convert go.untyped_bool go.bool ((![go.error] "err") ≠⟨go.error⟩ (Convert go.untyped_nil go.error UntypedNil))
               then
-                return: (Convert go.untyped_nil (go.InterfaceType []) UntypedNil, Convert (go.PointerType errors.StatusError) go.error (let: "$a0" := (let: "$a0" := #"failed to convert appsv1.Deployment to internal Deployment: %v"%go in
+                return: (Convert go.untyped_nil (go.InterfaceType []) UntypedNil, Convert (go.PointerType errors.StatusError) go.error (let: "$a0" := (let: "$a0" := #"failed to convert appsv1.StatefulSet to internal StatefulSet: %v"%go in
                  let: "$a1" := ((let: "$sl0" := (Convert go.error go.any (![go.error] "err")) in
                  CompositeLiteral (go.SliceType go.any) (LiteralValue [KeyedElement None (ElementExpression go.any "$sl0")]))) in
                  (FuncResolve fmt.Sprintf [] #()) "$a0" "$a1") in
                  (FuncResolve errors.NewBadRequest [] #()) "$a0"))
               else do:  #()));;;
-              return: (Convert (go.PointerType apps.Deployment) (go.InterfaceType []) (![go.PointerType apps.Deployment] "internalDeployment"), Convert go.untyped_nil go.error UntypedNil)
+              return: (Convert (go.PointerType apps.StatefulSet) (go.InterfaceType []) (![go.PointerType apps.StatefulSet] "internalSTS"), Convert go.untyped_nil go.error UntypedNil)
             else
-              return: (Convert go.untyped_nil (go.InterfaceType []) UntypedNil, let: "$a0" := #"unsupported versioned object type for conversion: %T"%go in
-               let: "$a1" := ((let: "$sl0" := (![go.InterfaceType []] "obj") in
-               CompositeLiteral (go.SliceType go.any) (LiteralValue [KeyedElement None (ElementExpression go.any "$sl0")]))) in
-               (FuncResolve fmt.Errorf [] #()) "$a0" "$a1"))))))).
+              let: ("$x", "$ok") := (TypeAssert2 (go.PointerType api_apps_v1.Deployment) "$y") in
+              (if: "$ok"
+              then
+                let: "typed" := (GoAlloc (go.PointerType api_apps_v1.Deployment) "$x") in
+                let: "internalDeployment" := (GoAlloc (go.PointerType apps.Deployment) (GoZeroVal (go.PointerType apps.Deployment) #())) in
+                let: "$r0" := (GoAlloc apps.Deployment (CompositeLiteral apps.Deployment (LiteralValue []))) in
+                do:  ("internalDeployment" <-[go.PointerType apps.Deployment] "$r0");;;
+                (let: "err" := (GoAlloc go.error (GoZeroVal go.error #())) in
+                let: "$r0" := (let: "$a0" := (Convert (go.PointerType api_apps_v1.Deployment) (go.InterfaceType []) (![go.PointerType api_apps_v1.Deployment] "typed")) in
+                let: "$a1" := (Convert (go.PointerType apps.Deployment) (go.InterfaceType []) (![go.PointerType apps.Deployment] "internalDeployment")) in
+                let: "$a2" := (Convert go.untyped_nil (go.InterfaceType []) UntypedNil) in
+                (MethodResolve (go.PointerType runtime.Scheme) "Convert"%go (![go.PointerType runtime.Scheme] (GlobalVarAddr legacyscheme.Scheme #()))) "$a0" "$a1" "$a2") in
+                do:  ("err" <-[go.error] "$r0");;;
+                (if: Convert go.untyped_bool go.bool ((![go.error] "err") ≠⟨go.error⟩ (Convert go.untyped_nil go.error UntypedNil))
+                then
+                  return: (Convert go.untyped_nil (go.InterfaceType []) UntypedNil, Convert (go.PointerType errors.StatusError) go.error (let: "$a0" := (let: "$a0" := #"failed to convert appsv1.Deployment to internal Deployment: %v"%go in
+                   let: "$a1" := ((let: "$sl0" := (Convert go.error go.any (![go.error] "err")) in
+                   CompositeLiteral (go.SliceType go.any) (LiteralValue [KeyedElement None (ElementExpression go.any "$sl0")]))) in
+                   (FuncResolve fmt.Sprintf [] #()) "$a0" "$a1") in
+                   (FuncResolve errors.NewBadRequest [] #()) "$a0"))
+                else do:  #()));;;
+                return: (Convert (go.PointerType apps.Deployment) (go.InterfaceType []) (![go.PointerType apps.Deployment] "internalDeployment"), Convert go.untyped_nil go.error UntypedNil)
+              else
+                return: (Convert go.untyped_nil (go.InterfaceType []) UntypedNil, let: "$a0" := #"unsupported versioned object type for conversion: %T"%go in
+                 let: "$a1" := ((let: "$sl0" := (![go.InterfaceType []] "obj") in
+                 CompositeLiteral (go.SliceType go.any) (LiteralValue [KeyedElement None (ElementExpression go.any "$sl0")]))) in
+                 (FuncResolve fmt.Errorf [] #()) "$a0" "$a1")))))))).
 
 (* applySchemaDefaults applies schema-based defaults to the object.
    This matches the API server's defaulting behavior that happens during decoding.
    These defaults are applied BEFORE PrepareForCreate and validation.
 
-   go: api_model.go:416:6 *)
+   go: api_model.go:427:6 *)
 Definition applySchemaDefaultsⁱᵐᵖˡ {ext : ffi_syntax} {go_gctx : GoGlobalContext} : val :=
   λ: "obj",
     exception_do (let: "obj" := (GoAlloc (go.InterfaceType []) "obj") in
@@ -905,34 +941,40 @@ Definition applySchemaDefaultsⁱᵐᵖˡ {ext : ffi_syntax} {go_gctx : GoGlobal
         do:  (let: "$a0" := (![go.PointerType api_core_v1.PersistentVolumeClaim] "typed") in
         (FuncResolve apis_core_v1.SetObjectDefaults_PersistentVolumeClaim [] #()) "$a0")
       else
-        let: ("$x", "$ok") := (TypeAssert2 (go.PointerType api_apps_v1.ReplicaSet) "$y") in
+        let: ("$x", "$ok") := (TypeAssert2 (go.PointerType api_core_v1.ServiceAccount) "$y") in
         (if: "$ok"
         then
-          let: "typed" := (GoAlloc (go.PointerType api_apps_v1.ReplicaSet) "$x") in
-          do:  (let: "$a0" := (![go.PointerType api_apps_v1.ReplicaSet] "typed") in
-          (FuncResolve apis_apps_v1.SetObjectDefaults_ReplicaSet [] #()) "$a0")
+          let: "typed" := (GoAlloc (go.PointerType api_core_v1.ServiceAccount) "$x") in
+          return: (Convert go.untyped_nil go.error UntypedNil)
         else
-          let: ("$x", "$ok") := (TypeAssert2 (go.PointerType api_apps_v1.StatefulSet) "$y") in
+          let: ("$x", "$ok") := (TypeAssert2 (go.PointerType api_apps_v1.ReplicaSet) "$y") in
           (if: "$ok"
           then
-            let: "typed" := (GoAlloc (go.PointerType api_apps_v1.StatefulSet) "$x") in
-            do:  (let: "$a0" := (![go.PointerType api_apps_v1.StatefulSet] "typed") in
-            (FuncResolve apis_apps_v1.SetObjectDefaults_StatefulSet [] #()) "$a0")
+            let: "typed" := (GoAlloc (go.PointerType api_apps_v1.ReplicaSet) "$x") in
+            do:  (let: "$a0" := (![go.PointerType api_apps_v1.ReplicaSet] "typed") in
+            (FuncResolve apis_apps_v1.SetObjectDefaults_ReplicaSet [] #()) "$a0")
           else
-            let: ("$x", "$ok") := (TypeAssert2 (go.PointerType api_apps_v1.Deployment) "$y") in
+            let: ("$x", "$ok") := (TypeAssert2 (go.PointerType api_apps_v1.StatefulSet) "$y") in
             (if: "$ok"
             then
-              let: "typed" := (GoAlloc (go.PointerType api_apps_v1.Deployment) "$x") in
-              do:  (let: "$a0" := (![go.PointerType api_apps_v1.Deployment] "typed") in
-              (FuncResolve apis_apps_v1.SetObjectDefaults_Deployment [] #()) "$a0")
+              let: "typed" := (GoAlloc (go.PointerType api_apps_v1.StatefulSet) "$x") in
+              do:  (let: "$a0" := (![go.PointerType api_apps_v1.StatefulSet] "typed") in
+              (FuncResolve apis_apps_v1.SetObjectDefaults_StatefulSet [] #()) "$a0")
             else
-              return: (let: "$a0" := #"unsupported object type for schema defaults: %T"%go in
-               let: "$a1" := ((let: "$sl0" := (![go.InterfaceType []] "obj") in
-               CompositeLiteral (go.SliceType go.any) (LiteralValue [KeyedElement None (ElementExpression go.any "$sl0")]))) in
-               (FuncResolve fmt.Errorf [] #()) "$a0" "$a1"))))));;;
+              let: ("$x", "$ok") := (TypeAssert2 (go.PointerType api_apps_v1.Deployment) "$y") in
+              (if: "$ok"
+              then
+                let: "typed" := (GoAlloc (go.PointerType api_apps_v1.Deployment) "$x") in
+                do:  (let: "$a0" := (![go.PointerType api_apps_v1.Deployment] "typed") in
+                (FuncResolve apis_apps_v1.SetObjectDefaults_Deployment [] #()) "$a0")
+              else
+                return: (let: "$a0" := #"unsupported object type for schema defaults: %T"%go in
+                 let: "$a1" := ((let: "$sl0" := (![go.InterfaceType []] "obj") in
+                 CompositeLiteral (go.SliceType go.any) (LiteralValue [KeyedElement None (ElementExpression go.any "$sl0")]))) in
+                 (FuncResolve fmt.Errorf [] #()) "$a0" "$a1")))))));;;
     return: (Convert go.untyped_nil go.error UntypedNil)).
 
-(* go: api_model.go:441:6 *)
+(* go: api_model.go:455:6 *)
 Definition applyStrategyPrepareForCreateⁱᵐᵖˡ {ext : ffi_syntax} {go_gctx : GoGlobalContext} : val :=
   λ: "obj",
     exception_do (let: "obj" := (GoAlloc (go.InterfaceType []) "obj") in
@@ -956,37 +998,45 @@ Definition applyStrategyPrepareForCreateⁱᵐᵖˡ {ext : ffi_syntax} {go_gctx 
         let: "$a1" := (Convert (go.PointerType core.PersistentVolumeClaim) runtime.Object (![go.PointerType core.PersistentVolumeClaim] "typed")) in
         (MethodResolve (go.PointerType persistentvolumeclaim.persistentvolumeclaimStrategy) "PrepareForCreate"%go (GlobalVarAddr persistentvolumeclaim.Strategy #())) "$a0" "$a1")
       else
-        let: ("$x", "$ok") := (TypeAssert2 (go.PointerType apps.ReplicaSet) "$y") in
+        let: ("$x", "$ok") := (TypeAssert2 (go.PointerType core.ServiceAccount) "$y") in
         (if: "$ok"
         then
-          let: "typed" := (GoAlloc (go.PointerType apps.ReplicaSet) "$x") in
+          let: "typed" := (GoAlloc (go.PointerType core.ServiceAccount) "$x") in
           do:  (let: "$a0" := (![context.Context] "ctx") in
-          let: "$a1" := (Convert (go.PointerType apps.ReplicaSet) runtime.Object (![go.PointerType apps.ReplicaSet] "typed")) in
-          (MethodResolve (go.PointerType replicaset.rsStrategy) "PrepareForCreate"%go (GlobalVarAddr replicaset.Strategy #())) "$a0" "$a1")
+          let: "$a1" := (Convert (go.PointerType core.ServiceAccount) runtime.Object (![go.PointerType core.ServiceAccount] "typed")) in
+          (MethodResolve (go.PointerType serviceaccount.strategy) "PrepareForCreate"%go (GlobalVarAddr serviceaccount.Strategy #())) "$a0" "$a1")
         else
-          let: ("$x", "$ok") := (TypeAssert2 (go.PointerType apps.StatefulSet) "$y") in
+          let: ("$x", "$ok") := (TypeAssert2 (go.PointerType apps.ReplicaSet) "$y") in
           (if: "$ok"
           then
-            let: "typed" := (GoAlloc (go.PointerType apps.StatefulSet) "$x") in
+            let: "typed" := (GoAlloc (go.PointerType apps.ReplicaSet) "$x") in
             do:  (let: "$a0" := (![context.Context] "ctx") in
-            let: "$a1" := (Convert (go.PointerType apps.StatefulSet) runtime.Object (![go.PointerType apps.StatefulSet] "typed")) in
-            (MethodResolve (go.PointerType statefulset.statefulSetStrategy) "PrepareForCreate"%go (GlobalVarAddr statefulset.Strategy #())) "$a0" "$a1")
+            let: "$a1" := (Convert (go.PointerType apps.ReplicaSet) runtime.Object (![go.PointerType apps.ReplicaSet] "typed")) in
+            (MethodResolve (go.PointerType replicaset.rsStrategy) "PrepareForCreate"%go (GlobalVarAddr replicaset.Strategy #())) "$a0" "$a1")
           else
-            let: ("$x", "$ok") := (TypeAssert2 (go.PointerType apps.Deployment) "$y") in
+            let: ("$x", "$ok") := (TypeAssert2 (go.PointerType apps.StatefulSet) "$y") in
             (if: "$ok"
             then
-              let: "typed" := (GoAlloc (go.PointerType apps.Deployment) "$x") in
+              let: "typed" := (GoAlloc (go.PointerType apps.StatefulSet) "$x") in
               do:  (let: "$a0" := (![context.Context] "ctx") in
-              let: "$a1" := (Convert (go.PointerType apps.Deployment) runtime.Object (![go.PointerType apps.Deployment] "typed")) in
-              (MethodResolve (go.PointerType deployment.deploymentStrategy) "PrepareForCreate"%go (GlobalVarAddr deployment.Strategy #())) "$a0" "$a1")
+              let: "$a1" := (Convert (go.PointerType apps.StatefulSet) runtime.Object (![go.PointerType apps.StatefulSet] "typed")) in
+              (MethodResolve (go.PointerType statefulset.statefulSetStrategy) "PrepareForCreate"%go (GlobalVarAddr statefulset.Strategy #())) "$a0" "$a1")
             else
-              return: (let: "$a0" := #"unsupported object type for strategy and validation: %T"%go in
-               let: "$a1" := ((let: "$sl0" := (![go.InterfaceType []] "obj") in
-               CompositeLiteral (go.SliceType go.any) (LiteralValue [KeyedElement None (ElementExpression go.any "$sl0")]))) in
-               (FuncResolve fmt.Errorf [] #()) "$a0" "$a1"))))));;;
+              let: ("$x", "$ok") := (TypeAssert2 (go.PointerType apps.Deployment) "$y") in
+              (if: "$ok"
+              then
+                let: "typed" := (GoAlloc (go.PointerType apps.Deployment) "$x") in
+                do:  (let: "$a0" := (![context.Context] "ctx") in
+                let: "$a1" := (Convert (go.PointerType apps.Deployment) runtime.Object (![go.PointerType apps.Deployment] "typed")) in
+                (MethodResolve (go.PointerType deployment.deploymentStrategy) "PrepareForCreate"%go (GlobalVarAddr deployment.Strategy #())) "$a0" "$a1")
+              else
+                return: (let: "$a0" := #"unsupported object type for strategy and validation: %T"%go in
+                 let: "$a1" := ((let: "$sl0" := (![go.InterfaceType []] "obj") in
+                 CompositeLiteral (go.SliceType go.any) (LiteralValue [KeyedElement None (ElementExpression go.any "$sl0")]))) in
+                 (FuncResolve fmt.Errorf [] #()) "$a0" "$a1")))))));;;
     return: (Convert go.untyped_nil go.error UntypedNil)).
 
-(* go: api_model.go:460:6 *)
+(* go: api_model.go:476:6 *)
 Definition applyAdmissionMutateⁱᵐᵖˡ {ext : ffi_syntax} {go_gctx : GoGlobalContext} : val :=
   λ: "obj",
     exception_do (let: "obj" := (GoAlloc (go.InterfaceType []) "obj") in
@@ -1007,28 +1057,34 @@ Definition applyAdmissionMutateⁱᵐᵖˡ {ext : ffi_syntax} {go_gctx : GoGloba
         do:  (let: "$a0" := (![go.PointerType core.PersistentVolumeClaim] "typed") in
         (FuncResolve applyPersistentVolumeClaimProtectionAdmission [] #()) "$a0")
       else
-        let: ("$x", "$ok") := (TypeAssert2 (go.PointerType apps.ReplicaSet) "$y") in
+        let: ("$x", "$ok") := (TypeAssert2 (go.PointerType core.ServiceAccount) "$y") in
         (if: "$ok"
         then
-          let: "typed" := (GoAlloc (go.PointerType apps.ReplicaSet) "$x") in
+          let: "typed" := (GoAlloc (go.PointerType core.ServiceAccount) "$x") in
           return: (Convert go.untyped_nil go.error UntypedNil)
         else
-          let: ("$x", "$ok") := (TypeAssert2 (go.PointerType apps.StatefulSet) "$y") in
+          let: ("$x", "$ok") := (TypeAssert2 (go.PointerType apps.ReplicaSet) "$y") in
           (if: "$ok"
           then
-            let: "typed" := (GoAlloc (go.PointerType apps.StatefulSet) "$x") in
+            let: "typed" := (GoAlloc (go.PointerType apps.ReplicaSet) "$x") in
             return: (Convert go.untyped_nil go.error UntypedNil)
           else
-            let: ("$x", "$ok") := (TypeAssert2 (go.PointerType apps.Deployment) "$y") in
+            let: ("$x", "$ok") := (TypeAssert2 (go.PointerType apps.StatefulSet) "$y") in
             (if: "$ok"
             then
-              let: "typed" := (GoAlloc (go.PointerType apps.Deployment) "$x") in
+              let: "typed" := (GoAlloc (go.PointerType apps.StatefulSet) "$x") in
               return: (Convert go.untyped_nil go.error UntypedNil)
             else
-              return: (let: "$a0" := #"unsupported object type for strategy and validation: %T"%go in
-               let: "$a1" := ((let: "$sl0" := (![go.InterfaceType []] "obj") in
-               CompositeLiteral (go.SliceType go.any) (LiteralValue [KeyedElement None (ElementExpression go.any "$sl0")]))) in
-               (FuncResolve fmt.Errorf [] #()) "$a0" "$a1"))))));;;
+              let: ("$x", "$ok") := (TypeAssert2 (go.PointerType apps.Deployment) "$y") in
+              (if: "$ok"
+              then
+                let: "typed" := (GoAlloc (go.PointerType apps.Deployment) "$x") in
+                return: (Convert go.untyped_nil go.error UntypedNil)
+              else
+                return: (let: "$a0" := #"unsupported object type for strategy and validation: %T"%go in
+                 let: "$a1" := ((let: "$sl0" := (![go.InterfaceType []] "obj") in
+                 CompositeLiteral (go.SliceType go.any) (LiteralValue [KeyedElement None (ElementExpression go.any "$sl0")]))) in
+                 (FuncResolve fmt.Errorf [] #()) "$a0" "$a1")))))));;;
     return: (Convert go.untyped_nil go.error UntypedNil)).
 
 (* applyPersistentVolumeClaimProtectionAdmission mirrors the built-in
@@ -1036,7 +1092,7 @@ Definition applyAdmissionMutateⁱᵐᵖˡ {ext : ffi_syntax} {go_gctx : GoGloba
    PVC creates, and the finalizer affects later delete behavior, so the model
    needs to store it rather than treating it as ignorable metadata.
 
-   go: api_model.go:486:6 *)
+   go: api_model.go:504:6 *)
 Definition applyPersistentVolumeClaimProtectionAdmissionⁱᵐᵖˡ {ext : ffi_syntax} {go_gctx : GoGlobalContext} : val :=
   λ: "pvc",
     exception_do (let: "pvc" := (GoAlloc (go.PointerType core.PersistentVolumeClaim) "pvc") in
@@ -1061,7 +1117,7 @@ Definition applyPersistentVolumeClaimProtectionAdmissionⁱᵐᵖˡ {ext : ffi_s
    initially sets status.phase=Pending, then the PVC strategy clears Status; the
    API server still stores and returns a created PVC with Pending phase.
 
-   go: api_model.go:500:6 *)
+   go: api_model.go:518:6 *)
 Definition applyPostPrepareCreateDefaultsⁱᵐᵖˡ {ext : ffi_syntax} {go_gctx : GoGlobalContext} : val :=
   λ: "obj",
     exception_do (let: "obj" := (GoAlloc (go.InterfaceType []) "obj") in
@@ -1082,28 +1138,34 @@ Definition applyPostPrepareCreateDefaultsⁱᵐᵖˡ {ext : ffi_syntax} {go_gctx
           do:  ((StructFieldRef core.PersistentVolumeClaimStatus "Phase"%go (StructFieldRef core.PersistentVolumeClaim "Status"%go (![go.PointerType core.PersistentVolumeClaim] "typed"))) <-[core.PersistentVolumeClaimPhase] "$r0")
         else do:  #())
       else
-        let: ("$x", "$ok") := (TypeAssert2 (go.PointerType apps.ReplicaSet) "$y") in
+        let: ("$x", "$ok") := (TypeAssert2 (go.PointerType core.ServiceAccount) "$y") in
         (if: "$ok"
         then
-          let: "typed" := (GoAlloc (go.PointerType apps.ReplicaSet) "$x") in
+          let: "typed" := (GoAlloc (go.PointerType core.ServiceAccount) "$x") in
           return: (Convert go.untyped_nil go.error UntypedNil)
         else
-          let: ("$x", "$ok") := (TypeAssert2 (go.PointerType apps.StatefulSet) "$y") in
+          let: ("$x", "$ok") := (TypeAssert2 (go.PointerType apps.ReplicaSet) "$y") in
           (if: "$ok"
           then
-            let: "typed" := (GoAlloc (go.PointerType apps.StatefulSet) "$x") in
+            let: "typed" := (GoAlloc (go.PointerType apps.ReplicaSet) "$x") in
             return: (Convert go.untyped_nil go.error UntypedNil)
           else
-            let: ("$x", "$ok") := (TypeAssert2 (go.PointerType apps.Deployment) "$y") in
+            let: ("$x", "$ok") := (TypeAssert2 (go.PointerType apps.StatefulSet) "$y") in
             (if: "$ok"
             then
-              let: "typed" := (GoAlloc (go.PointerType apps.Deployment) "$x") in
+              let: "typed" := (GoAlloc (go.PointerType apps.StatefulSet) "$x") in
               return: (Convert go.untyped_nil go.error UntypedNil)
             else
-              return: (let: "$a0" := #"unsupported object type for post-prepare create defaults: %T"%go in
-               let: "$a1" := ((let: "$sl0" := (![go.InterfaceType []] "obj") in
-               CompositeLiteral (go.SliceType go.any) (LiteralValue [KeyedElement None (ElementExpression go.any "$sl0")]))) in
-               (FuncResolve fmt.Errorf [] #()) "$a0" "$a1"))))));;;
+              let: ("$x", "$ok") := (TypeAssert2 (go.PointerType apps.Deployment) "$y") in
+              (if: "$ok"
+              then
+                let: "typed" := (GoAlloc (go.PointerType apps.Deployment) "$x") in
+                return: (Convert go.untyped_nil go.error UntypedNil)
+              else
+                return: (let: "$a0" := #"unsupported object type for post-prepare create defaults: %T"%go in
+                 let: "$a1" := ((let: "$sl0" := (![go.InterfaceType []] "obj") in
+                 CompositeLiteral (go.SliceType go.any) (LiteralValue [KeyedElement None (ElementExpression go.any "$sl0")]))) in
+                 (FuncResolve fmt.Errorf [] #()) "$a0" "$a1")))))));;;
     return: (Convert go.untyped_nil go.error UntypedNil)).
 
 (* normalizeVersionedObject removes conversion artifacts after converting an
@@ -1111,7 +1173,7 @@ Definition applyPostPrepareCreateDefaultsⁱᵐᵖˡ {ext : ffi_syntax} {go_gctx
    not store TypeMeta on StatefulSet volumeClaimTemplates, while the internal to
    external conversion can materialize kind/apiVersion on those embedded PVCs.
 
-   go: api_model.go:524:6 *)
+   go: api_model.go:544:6 *)
 Definition normalizeVersionedObjectⁱᵐᵖˡ {ext : ffi_syntax} {go_gctx : GoGlobalContext} : val :=
   λ: "obj",
     exception_do (let: "obj" := (GoAlloc (go.InterfaceType []) "obj") in
@@ -1136,7 +1198,7 @@ Definition normalizeVersionedObjectⁱᵐᵖˡ {ext : ffi_syntax} {go_gctx : GoG
    - https://github.com/kubernetes/kubernetes/blob/release-1.34/plugin/pkg/admission/defaulttolerationseconds/admission.go#L107-L145
    - https://github.com/kubernetes/kubernetes/blob/release-1.34/plugin/pkg/admission/priority/admission.go#L136-L158
 
-   go: api_model.go:539:6 *)
+   go: api_model.go:559:6 *)
 Definition applyAdmissionMutateForUpdateⁱᵐᵖˡ {ext : ffi_syntax} {go_gctx : GoGlobalContext} : val :=
   λ: "obj" "oldObj",
     exception_do (let: "oldObj" := (GoAlloc (go.InterfaceType []) "oldObj") in
@@ -1209,7 +1271,7 @@ Definition applyAdmissionMutateForUpdateⁱᵐᵖˡ {ext : ffi_syntax} {go_gctx 
                (FuncResolve fmt.Errorf [] #()) "$a0" "$a1"))))));;;
     return: (Convert go.untyped_nil go.error UntypedNil)).
 
-(* go: api_model.go:572:6 *)
+(* go: api_model.go:592:6 *)
 Definition applyAdmissionValidateⁱᵐᵖˡ {ext : ffi_syntax} {go_gctx : GoGlobalContext} : val :=
   λ: "obj",
     exception_do (let: "obj" := (GoAlloc (go.InterfaceType []) "obj") in
@@ -1222,24 +1284,28 @@ Definition applyAdmissionValidateⁱᵐᵖˡ {ext : ffi_syntax} {go_gctx : GoGlo
       (if: "$ok"
       then return: (Convert go.untyped_nil go.error UntypedNil)
       else
-        let: ("$x", "$ok") := (TypeAssert2 (go.PointerType apps.ReplicaSet) "$y") in
+        let: ("$x", "$ok") := (TypeAssert2 (go.PointerType core.ServiceAccount) "$y") in
         (if: "$ok"
         then return: (Convert go.untyped_nil go.error UntypedNil)
         else
-          let: ("$x", "$ok") := (TypeAssert2 (go.PointerType apps.StatefulSet) "$y") in
+          let: ("$x", "$ok") := (TypeAssert2 (go.PointerType apps.ReplicaSet) "$y") in
           (if: "$ok"
           then return: (Convert go.untyped_nil go.error UntypedNil)
           else
-            let: ("$x", "$ok") := (TypeAssert2 (go.PointerType apps.Deployment) "$y") in
+            let: ("$x", "$ok") := (TypeAssert2 (go.PointerType apps.StatefulSet) "$y") in
             (if: "$ok"
             then return: (Convert go.untyped_nil go.error UntypedNil)
             else
-              return: (let: "$a0" := #"unsupported object type for admission validation: %T"%go in
-               let: "$a1" := ((let: "$sl0" := (![go.InterfaceType []] "obj") in
-               CompositeLiteral (go.SliceType go.any) (LiteralValue [KeyedElement None (ElementExpression go.any "$sl0")]))) in
-               (FuncResolve fmt.Errorf [] #()) "$a0" "$a1"))))))).
+              let: ("$x", "$ok") := (TypeAssert2 (go.PointerType apps.Deployment) "$y") in
+              (if: "$ok"
+              then return: (Convert go.untyped_nil go.error UntypedNil)
+              else
+                return: (let: "$a0" := #"unsupported object type for admission validation: %T"%go in
+                 let: "$a1" := ((let: "$sl0" := (![go.InterfaceType []] "obj") in
+                 CompositeLiteral (go.SliceType go.any) (LiteralValue [KeyedElement None (ElementExpression go.any "$sl0")]))) in
+                 (FuncResolve fmt.Errorf [] #()) "$a0" "$a1")))))))).
 
-(* go: api_model.go:597:6 *)
+(* go: api_model.go:620:6 *)
 Definition allowUnconditionalUpdateⁱᵐᵖˡ {ext : ffi_syntax} {go_gctx : GoGlobalContext} : val :=
   λ: "kind",
     exception_do (let: "kind" := (GoAlloc go.string "kind") in
@@ -1252,7 +1318,7 @@ Definition allowUnconditionalUpdateⁱᵐᵖˡ {ext : ffi_syntax} {go_gctx : GoG
        CompositeLiteral (go.SliceType go.any) (LiteralValue [KeyedElement None (ElementExpression go.any "$sl0")]))) in
        (FuncResolve fmt.Errorf [] #()) "$a0" "$a1"))).
 
-(* go: api_model.go:613:6 *)
+(* go: api_model.go:636:6 *)
 Definition malformedUpdateResourceVersionErrorⁱᵐᵖˡ {ext : ffi_syntax} {go_gctx : GoGlobalContext} : val :=
   λ: "err",
     exception_do (let: "err" := (GoAlloc go.error "err") in
@@ -1262,7 +1328,7 @@ Definition malformedUpdateResourceVersionErrorⁱᵐᵖˡ {ext : ffi_syntax} {go
      CompositeLiteral apis_meta_v1.Status (LiteralValue [KeyedElement (Some (KeyField "Status"%go)) (ElementExpression go.string "$v0"); KeyedElement (Some (KeyField "Code"%go)) (ElementExpression go.int32 "$v1"); KeyedElement (Some (KeyField "Message"%go)) (ElementExpression go.string "$v2")])) in
      CompositeLiteral errors.StatusError (LiteralValue [KeyedElement (Some (KeyField "ErrStatus"%go)) (ElementExpression apis_meta_v1.Status "$v0")]))))).
 
-(* go: api_model.go:621:6 *)
+(* go: api_model.go:644:6 *)
 Definition parseResourceVersionⁱᵐᵖˡ {ext : ffi_syntax} {go_gctx : GoGlobalContext} : val :=
   λ: "resourceVersion",
     exception_do (let: "resourceVersion" := (GoAlloc go.string "resourceVersion") in
@@ -1272,7 +1338,7 @@ Definition parseResourceVersionⁱᵐᵖˡ {ext : ffi_syntax} {go_gctx : GoGloba
     (FuncResolve strconv.ParseUint [] #()) "$a0" "$a1" "$a2")) in
     return: ("$ret0", "$ret1")).
 
-(* go: api_model.go:625:6 *)
+(* go: api_model.go:648:6 *)
 Definition updateStrategyForLegacyObjectⁱᵐᵖˡ {ext : ffi_syntax} {go_gctx : GoGlobalContext} : val :=
   λ: "obj",
     exception_do (let: "obj" := (GoAlloc (go.InterfaceType []) "obj") in
@@ -1302,7 +1368,7 @@ Definition updateStrategyForLegacyObjectⁱᵐᵖˡ {ext : ffi_syntax} {go_gctx 
                CompositeLiteral (go.SliceType go.any) (LiteralValue [KeyedElement None (ElementExpression go.any "$sl0")]))) in
                (FuncResolve fmt.Errorf [] #()) "$a0" "$a1"))))))).
 
-(* go: api_model.go:642:6 *)
+(* go: api_model.go:665:6 *)
 Definition statusUpdateStrategyForLegacyObjectⁱᵐᵖˡ {ext : ffi_syntax} {go_gctx : GoGlobalContext} : val :=
   λ: "obj",
     exception_do (let: "obj" := (GoAlloc (go.InterfaceType []) "obj") in
@@ -1332,7 +1398,7 @@ Definition statusUpdateStrategyForLegacyObjectⁱᵐᵖˡ {ext : ffi_syntax} {go
                CompositeLiteral (go.SliceType go.any) (LiteralValue [KeyedElement None (ElementExpression go.any "$sl0")]))) in
                (FuncResolve fmt.Errorf [] #()) "$a0" "$a1"))))))).
 
-(* go: api_model.go:659:6 *)
+(* go: api_model.go:682:6 *)
 Definition applyStrategyValidateⁱᵐᵖˡ {ext : ffi_syntax} {go_gctx : GoGlobalContext} : val :=
   λ: "obj" "name",
     exception_do (let: "name" := (GoAlloc go.string "name") in
@@ -1381,73 +1447,93 @@ Definition applyStrategyValidateⁱᵐᵖˡ {ext : ffi_syntax} {go_gctx : GoGlob
            (FuncResolve errors.NewInvalid [] #()) "$a0" "$a1" "$a2"))
         else do:  #()))
       else
-        let: ("$x", "$ok") := (TypeAssert2 (go.PointerType apps.ReplicaSet) "$y") in
+        let: ("$x", "$ok") := (TypeAssert2 (go.PointerType core.ServiceAccount) "$y") in
         (if: "$ok"
         then
-          let: "typed" := (GoAlloc (go.PointerType apps.ReplicaSet) "$x") in
+          let: "typed" := (GoAlloc (go.PointerType core.ServiceAccount) "$x") in
           (let: "errs" := (GoAlloc field.ErrorList (GoZeroVal field.ErrorList #())) in
           let: "$r0" := (let: "$a0" := (![context.Context] "ctx") in
-          let: "$a1" := (Convert (go.PointerType apps.ReplicaSet) runtime.Object (![go.PointerType apps.ReplicaSet] "typed")) in
-          (MethodResolve (go.PointerType replicaset.rsStrategy) "Validate"%go (GlobalVarAddr replicaset.Strategy #())) "$a0" "$a1") in
+          let: "$a1" := (Convert (go.PointerType core.ServiceAccount) runtime.Object (![go.PointerType core.ServiceAccount] "typed")) in
+          (MethodResolve (go.PointerType serviceaccount.strategy) "Validate"%go (GlobalVarAddr serviceaccount.Strategy #())) "$a0" "$a1") in
           do:  ("errs" <-[field.ErrorList] "$r0");;;
           (if: Convert go.untyped_bool go.bool ((let: "$a0" := (![field.ErrorList] "errs") in
           (FuncResolve go.len [field.ErrorList] #()) "$a0") >⟨go.int⟩ #(W64 0))
           then
-            return: (Convert (go.PointerType errors.StatusError) go.error (let: "$a0" := (let: "$v0" := #"apps"%go in
-             let: "$v1" := #"ReplicaSet"%go in
+            return: (Convert (go.PointerType errors.StatusError) go.error (let: "$a0" := (let: "$v0" := #""%go in
+             let: "$v1" := #"ServiceAccount"%go in
              CompositeLiteral schema.GroupKind (LiteralValue [KeyedElement (Some (KeyField "Group"%go)) (ElementExpression go.string "$v0"); KeyedElement (Some (KeyField "Kind"%go)) (ElementExpression go.string "$v1")])) in
              let: "$a1" := (![go.string] "name") in
              let: "$a2" := (![field.ErrorList] "errs") in
              (FuncResolve errors.NewInvalid [] #()) "$a0" "$a1" "$a2"))
           else do:  #()))
         else
-          let: ("$x", "$ok") := (TypeAssert2 (go.PointerType apps.StatefulSet) "$y") in
+          let: ("$x", "$ok") := (TypeAssert2 (go.PointerType apps.ReplicaSet) "$y") in
           (if: "$ok"
           then
-            let: "typed" := (GoAlloc (go.PointerType apps.StatefulSet) "$x") in
+            let: "typed" := (GoAlloc (go.PointerType apps.ReplicaSet) "$x") in
             (let: "errs" := (GoAlloc field.ErrorList (GoZeroVal field.ErrorList #())) in
             let: "$r0" := (let: "$a0" := (![context.Context] "ctx") in
-            let: "$a1" := (Convert (go.PointerType apps.StatefulSet) runtime.Object (![go.PointerType apps.StatefulSet] "typed")) in
-            (MethodResolve (go.PointerType statefulset.statefulSetStrategy) "Validate"%go (GlobalVarAddr statefulset.Strategy #())) "$a0" "$a1") in
+            let: "$a1" := (Convert (go.PointerType apps.ReplicaSet) runtime.Object (![go.PointerType apps.ReplicaSet] "typed")) in
+            (MethodResolve (go.PointerType replicaset.rsStrategy) "Validate"%go (GlobalVarAddr replicaset.Strategy #())) "$a0" "$a1") in
             do:  ("errs" <-[field.ErrorList] "$r0");;;
             (if: Convert go.untyped_bool go.bool ((let: "$a0" := (![field.ErrorList] "errs") in
             (FuncResolve go.len [field.ErrorList] #()) "$a0") >⟨go.int⟩ #(W64 0))
             then
               return: (Convert (go.PointerType errors.StatusError) go.error (let: "$a0" := (let: "$v0" := #"apps"%go in
-               let: "$v1" := #"StatefulSet"%go in
+               let: "$v1" := #"ReplicaSet"%go in
                CompositeLiteral schema.GroupKind (LiteralValue [KeyedElement (Some (KeyField "Group"%go)) (ElementExpression go.string "$v0"); KeyedElement (Some (KeyField "Kind"%go)) (ElementExpression go.string "$v1")])) in
                let: "$a1" := (![go.string] "name") in
                let: "$a2" := (![field.ErrorList] "errs") in
                (FuncResolve errors.NewInvalid [] #()) "$a0" "$a1" "$a2"))
             else do:  #()))
           else
-            let: ("$x", "$ok") := (TypeAssert2 (go.PointerType apps.Deployment) "$y") in
+            let: ("$x", "$ok") := (TypeAssert2 (go.PointerType apps.StatefulSet) "$y") in
             (if: "$ok"
             then
-              let: "typed" := (GoAlloc (go.PointerType apps.Deployment) "$x") in
+              let: "typed" := (GoAlloc (go.PointerType apps.StatefulSet) "$x") in
               (let: "errs" := (GoAlloc field.ErrorList (GoZeroVal field.ErrorList #())) in
               let: "$r0" := (let: "$a0" := (![context.Context] "ctx") in
-              let: "$a1" := (Convert (go.PointerType apps.Deployment) runtime.Object (![go.PointerType apps.Deployment] "typed")) in
-              (MethodResolve (go.PointerType deployment.deploymentStrategy) "Validate"%go (GlobalVarAddr deployment.Strategy #())) "$a0" "$a1") in
+              let: "$a1" := (Convert (go.PointerType apps.StatefulSet) runtime.Object (![go.PointerType apps.StatefulSet] "typed")) in
+              (MethodResolve (go.PointerType statefulset.statefulSetStrategy) "Validate"%go (GlobalVarAddr statefulset.Strategy #())) "$a0" "$a1") in
               do:  ("errs" <-[field.ErrorList] "$r0");;;
               (if: Convert go.untyped_bool go.bool ((let: "$a0" := (![field.ErrorList] "errs") in
               (FuncResolve go.len [field.ErrorList] #()) "$a0") >⟨go.int⟩ #(W64 0))
               then
                 return: (Convert (go.PointerType errors.StatusError) go.error (let: "$a0" := (let: "$v0" := #"apps"%go in
-                 let: "$v1" := #"Deployment"%go in
+                 let: "$v1" := #"StatefulSet"%go in
                  CompositeLiteral schema.GroupKind (LiteralValue [KeyedElement (Some (KeyField "Group"%go)) (ElementExpression go.string "$v0"); KeyedElement (Some (KeyField "Kind"%go)) (ElementExpression go.string "$v1")])) in
                  let: "$a1" := (![go.string] "name") in
                  let: "$a2" := (![field.ErrorList] "errs") in
                  (FuncResolve errors.NewInvalid [] #()) "$a0" "$a1" "$a2"))
               else do:  #()))
             else
-              return: (let: "$a0" := #"unsupported object type for strategy and validation: %T"%go in
-               let: "$a1" := ((let: "$sl0" := (![go.InterfaceType []] "obj") in
-               CompositeLiteral (go.SliceType go.any) (LiteralValue [KeyedElement None (ElementExpression go.any "$sl0")]))) in
-               (FuncResolve fmt.Errorf [] #()) "$a0" "$a1"))))));;;
+              let: ("$x", "$ok") := (TypeAssert2 (go.PointerType apps.Deployment) "$y") in
+              (if: "$ok"
+              then
+                let: "typed" := (GoAlloc (go.PointerType apps.Deployment) "$x") in
+                (let: "errs" := (GoAlloc field.ErrorList (GoZeroVal field.ErrorList #())) in
+                let: "$r0" := (let: "$a0" := (![context.Context] "ctx") in
+                let: "$a1" := (Convert (go.PointerType apps.Deployment) runtime.Object (![go.PointerType apps.Deployment] "typed")) in
+                (MethodResolve (go.PointerType deployment.deploymentStrategy) "Validate"%go (GlobalVarAddr deployment.Strategy #())) "$a0" "$a1") in
+                do:  ("errs" <-[field.ErrorList] "$r0");;;
+                (if: Convert go.untyped_bool go.bool ((let: "$a0" := (![field.ErrorList] "errs") in
+                (FuncResolve go.len [field.ErrorList] #()) "$a0") >⟨go.int⟩ #(W64 0))
+                then
+                  return: (Convert (go.PointerType errors.StatusError) go.error (let: "$a0" := (let: "$v0" := #"apps"%go in
+                   let: "$v1" := #"Deployment"%go in
+                   CompositeLiteral schema.GroupKind (LiteralValue [KeyedElement (Some (KeyField "Group"%go)) (ElementExpression go.string "$v0"); KeyedElement (Some (KeyField "Kind"%go)) (ElementExpression go.string "$v1")])) in
+                   let: "$a1" := (![go.string] "name") in
+                   let: "$a2" := (![field.ErrorList] "errs") in
+                   (FuncResolve errors.NewInvalid [] #()) "$a0" "$a1" "$a2"))
+                else do:  #()))
+              else
+                return: (let: "$a0" := #"unsupported object type for strategy and validation: %T"%go in
+                 let: "$a1" := ((let: "$sl0" := (![go.InterfaceType []] "obj") in
+                 CompositeLiteral (go.SliceType go.any) (LiteralValue [KeyedElement None (ElementExpression go.any "$sl0")]))) in
+                 (FuncResolve fmt.Errorf [] #()) "$a0" "$a1")))))));;;
     return: (Convert go.untyped_nil go.error UntypedNil)).
 
-(* go: api_model.go:688:6 *)
+(* go: api_model.go:715:6 *)
 Definition applyStrategyCanonicalizeⁱᵐᵖˡ {ext : ffi_syntax} {go_gctx : GoGlobalContext} : val :=
   λ: "obj",
     exception_do (let: "obj" := (GoAlloc (go.InterfaceType []) "obj") in
@@ -1466,31 +1552,38 @@ Definition applyStrategyCanonicalizeⁱᵐᵖˡ {ext : ffi_syntax} {go_gctx : Go
         do:  (let: "$a0" := (Convert (go.PointerType core.PersistentVolumeClaim) runtime.Object (![go.PointerType core.PersistentVolumeClaim] "typed")) in
         (MethodResolve (go.PointerType persistentvolumeclaim.persistentvolumeclaimStrategy) "Canonicalize"%go (GlobalVarAddr persistentvolumeclaim.Strategy #())) "$a0")
       else
-        let: ("$x", "$ok") := (TypeAssert2 (go.PointerType apps.ReplicaSet) "$y") in
+        let: ("$x", "$ok") := (TypeAssert2 (go.PointerType core.ServiceAccount) "$y") in
         (if: "$ok"
         then
-          let: "typed" := (GoAlloc (go.PointerType apps.ReplicaSet) "$x") in
-          do:  (let: "$a0" := (Convert (go.PointerType apps.ReplicaSet) runtime.Object (![go.PointerType apps.ReplicaSet] "typed")) in
-          (MethodResolve (go.PointerType replicaset.rsStrategy) "Canonicalize"%go (GlobalVarAddr replicaset.Strategy #())) "$a0")
+          let: "typed" := (GoAlloc (go.PointerType core.ServiceAccount) "$x") in
+          do:  (let: "$a0" := (Convert (go.PointerType core.ServiceAccount) runtime.Object (![go.PointerType core.ServiceAccount] "typed")) in
+          (MethodResolve (go.PointerType serviceaccount.strategy) "Canonicalize"%go (GlobalVarAddr serviceaccount.Strategy #())) "$a0")
         else
-          let: ("$x", "$ok") := (TypeAssert2 (go.PointerType apps.StatefulSet) "$y") in
+          let: ("$x", "$ok") := (TypeAssert2 (go.PointerType apps.ReplicaSet) "$y") in
           (if: "$ok"
           then
-            let: "typed" := (GoAlloc (go.PointerType apps.StatefulSet) "$x") in
-            do:  (let: "$a0" := (Convert (go.PointerType apps.StatefulSet) runtime.Object (![go.PointerType apps.StatefulSet] "typed")) in
-            (MethodResolve (go.PointerType statefulset.statefulSetStrategy) "Canonicalize"%go (GlobalVarAddr statefulset.Strategy #())) "$a0")
+            let: "typed" := (GoAlloc (go.PointerType apps.ReplicaSet) "$x") in
+            do:  (let: "$a0" := (Convert (go.PointerType apps.ReplicaSet) runtime.Object (![go.PointerType apps.ReplicaSet] "typed")) in
+            (MethodResolve (go.PointerType replicaset.rsStrategy) "Canonicalize"%go (GlobalVarAddr replicaset.Strategy #())) "$a0")
           else
-            let: ("$x", "$ok") := (TypeAssert2 (go.PointerType apps.Deployment) "$y") in
+            let: ("$x", "$ok") := (TypeAssert2 (go.PointerType apps.StatefulSet) "$y") in
             (if: "$ok"
             then
-              let: "typed" := (GoAlloc (go.PointerType apps.Deployment) "$x") in
-              do:  (let: "$a0" := (Convert (go.PointerType apps.Deployment) runtime.Object (![go.PointerType apps.Deployment] "typed")) in
-              (MethodResolve (go.PointerType deployment.deploymentStrategy) "Canonicalize"%go (GlobalVarAddr deployment.Strategy #())) "$a0")
+              let: "typed" := (GoAlloc (go.PointerType apps.StatefulSet) "$x") in
+              do:  (let: "$a0" := (Convert (go.PointerType apps.StatefulSet) runtime.Object (![go.PointerType apps.StatefulSet] "typed")) in
+              (MethodResolve (go.PointerType statefulset.statefulSetStrategy) "Canonicalize"%go (GlobalVarAddr statefulset.Strategy #())) "$a0")
             else
-              return: (let: "$a0" := #"unsupported object type for strategy and validation: %T"%go in
-               let: "$a1" := ((let: "$sl0" := (![go.InterfaceType []] "obj") in
-               CompositeLiteral (go.SliceType go.any) (LiteralValue [KeyedElement None (ElementExpression go.any "$sl0")]))) in
-               (FuncResolve fmt.Errorf [] #()) "$a0" "$a1"))))));;;
+              let: ("$x", "$ok") := (TypeAssert2 (go.PointerType apps.Deployment) "$y") in
+              (if: "$ok"
+              then
+                let: "typed" := (GoAlloc (go.PointerType apps.Deployment) "$x") in
+                do:  (let: "$a0" := (Convert (go.PointerType apps.Deployment) runtime.Object (![go.PointerType apps.Deployment] "typed")) in
+                (MethodResolve (go.PointerType deployment.deploymentStrategy) "Canonicalize"%go (GlobalVarAddr deployment.Strategy #())) "$a0")
+              else
+                return: (let: "$a0" := #"unsupported object type for strategy and validation: %T"%go in
+                 let: "$a1" := ((let: "$sl0" := (![go.InterfaceType []] "obj") in
+                 CompositeLiteral (go.SliceType go.any) (LiteralValue [KeyedElement None (ElementExpression go.any "$sl0")]))) in
+                 (FuncResolve fmt.Errorf [] #()) "$a0" "$a1")))))));;;
     return: (Convert go.untyped_nil go.error UntypedNil)).
 
 (* applyValidationAndDefaultingOnUpdate models the decode/defaulting/admission/storage
@@ -1500,7 +1593,7 @@ Definition applyStrategyCanonicalizeⁱᵐᵖˡ {ext : ffi_syntax} {go_gctx : Go
    - https://github.com/kubernetes/kubernetes/blob/release-1.34/staging/src/k8s.io/apiserver/pkg/registry/rest/update.go#L107-L165
    - https://github.com/kubernetes/kubernetes/blob/release-1.34/staging/src/k8s.io/apiserver/pkg/registry/generic/registry/store.go#L753-L770
 
-   go: api_model.go:712:6 *)
+   go: api_model.go:741:6 *)
 Definition applyValidationAndDefaultingOnUpdateⁱᵐᵖˡ {ext : ffi_syntax} {go_gctx : GoGlobalContext} : val :=
   λ: "newObj" "oldObj" "namespace",
     exception_do (let: "namespace" := (GoAlloc go.string "namespace") in
@@ -1627,7 +1720,7 @@ Definition applyValidationAndDefaultingOnUpdateⁱᵐᵖˡ {ext : ffi_syntax} {g
    - https://github.com/kubernetes/kubernetes/blob/release-1.34/pkg/registry/apps/replicaset/storage/storage.go#L107-L109
    - https://github.com/kubernetes/kubernetes/blob/release-1.34/staging/src/k8s.io/apiserver/pkg/registry/rest/update.go#L107-L165
 
-   go: api_model.go:769:6 *)
+   go: api_model.go:798:6 *)
 Definition applyValidationAndDefaultingOnStatusUpdateⁱᵐᵖˡ {ext : ffi_syntax} {go_gctx : GoGlobalContext} : val :=
   λ: "newObj" "oldObj" "namespace",
     exception_do (let: "namespace" := (GoAlloc go.string "namespace") in
@@ -1738,7 +1831,7 @@ Definition applyValidationAndDefaultingOnStatusUpdateⁱᵐᵖˡ {ext : ffi_synt
     (FuncResolve normalizeVersionedObject [] #()) "$a0");;;
     return: (Convert go.untyped_nil go.error UntypedNil)).
 
-(* go: api_model.go:813:6 *)
+(* go: api_model.go:842:6 *)
 Definition applyValidationAndDefaultingⁱᵐᵖˡ {ext : ffi_syntax} {go_gctx : GoGlobalContext} : val :=
   λ: "obj" "name",
     exception_do (let: "name" := (GoAlloc go.string "name") in
@@ -1822,7 +1915,7 @@ Definition applyValidationAndDefaultingⁱᵐᵖˡ {ext : ffi_syntax} {go_gctx :
     (FuncResolve normalizeVersionedObject [] #()) "$a0");;;
     return: (Convert go.untyped_nil go.error UntypedNil)).
 
-(* go: api_model.go:872:17 *)
+(* go: api_model.go:901:17 *)
 Definition State__createⁱᵐᵖˡ {ext : ffi_syntax} {go_gctx : GoGlobalContext} : val :=
   λ: "s" "kind" "namespace" "obj",
     with_defer: (let: "s" := (GoAlloc (go.PointerType State) "s") in
@@ -1937,7 +2030,7 @@ Definition State__createⁱᵐᵖˡ {ext : ffi_syntax} {go_gctx : GoGlobalContex
    - https://github.com/kubernetes/kubernetes/blob/release-1.34/staging/src/k8s.io/apiserver/pkg/registry/generic/registry/store.go#L652-L777
    - https://github.com/kubernetes/kubernetes/blob/release-1.34/staging/src/k8s.io/apimachinery/pkg/api/validation/objectmeta.go#L233-L260
 
-   go: api_model.go:938:17 *)
+   go: api_model.go:967:17 *)
 Definition State__updateⁱᵐᵖˡ {ext : ffi_syntax} {go_gctx : GoGlobalContext} : val :=
   λ: "s" "kind" "namespace" "obj",
     with_defer: (let: "s" := (GoAlloc (go.PointerType State) "s") in
@@ -2125,7 +2218,7 @@ Definition State__updateⁱᵐᵖˡ {ext : ffi_syntax} {go_gctx : GoGlobalContex
     return: (let: "$a0" := (![go.InterfaceType []] "objCopy") in
      (FuncResolve deepCopy [] #()) "$a0", Convert go.untyped_nil go.error UntypedNil)).
 
-(* go: api_model.go:1038:17 *)
+(* go: api_model.go:1067:17 *)
 Definition State__updateStatusⁱᵐᵖˡ {ext : ffi_syntax} {go_gctx : GoGlobalContext} : val :=
   λ: "s" "kind" "namespace" "obj",
     with_defer: (let: "s" := (GoAlloc (go.PointerType State) "s") in
@@ -2316,7 +2409,7 @@ Definition State__updateStatusⁱᵐᵖˡ {ext : ffi_syntax} {go_gctx : GoGlobal
 (* shouldOrphanDependents determines if the orphan finalizer should be set based on DeleteOptions.
    Reference: https://github.com/kubernetes/kubernetes/blob/release-1.34/staging/src/k8s.io/apiserver/pkg/registry/generic/registry/store.go#L888-L925
 
-   go: api_model.go:1127:6 *)
+   go: api_model.go:1156:6 *)
 Definition shouldOrphanDependentsⁱᵐᵖˡ {ext : ffi_syntax} {go_gctx : GoGlobalContext} : val :=
   λ: "metadata" "options",
     exception_do (let: "options" := (GoAlloc (go.PointerType apis_meta_v1.DeleteOptions) "options") in
@@ -2354,7 +2447,7 @@ Definition shouldOrphanDependentsⁱᵐᵖˡ {ext : ffi_syntax} {go_gctx : GoGlo
 (* shouldDeleteDependents determines if the foreground deletion finalizer should be set based on DeleteOptions.
    Reference: https://github.com/kubernetes/kubernetes/blob/release-1.34/staging/src/k8s.io/apiserver/pkg/registry/generic/registry/store.go#L927-L966
 
-   go: api_model.go:1161:6 *)
+   go: api_model.go:1190:6 *)
 Definition shouldDeleteDependentsⁱᵐᵖˡ {ext : ffi_syntax} {go_gctx : GoGlobalContext} : val :=
   λ: "metadata" "options",
     exception_do (let: "options" := (GoAlloc (go.PointerType apis_meta_v1.DeleteOptions) "options") in
@@ -2393,7 +2486,7 @@ Definition shouldDeleteDependentsⁱᵐᵖˡ {ext : ffi_syntax} {go_gctx : GoGlo
    It returns whether the finalizer list needs updating and the new finalizer list.
    Reference: https://github.com/kubernetes/kubernetes/blob/release-1.34/staging/src/k8s.io/apiserver/pkg/registry/generic/registry/store.go#L976-L1005
 
-   go: api_model.go:1196:6 *)
+   go: api_model.go:1225:6 *)
 Definition deletionFinalizersForGarbageCollectionⁱᵐᵖˡ {ext : ffi_syntax} {go_gctx : GoGlobalContext} : val :=
   λ: "metadata" "options",
     exception_do (let: "options" := (GoAlloc (go.PointerType apis_meta_v1.DeleteOptions) "options") in
@@ -2468,7 +2561,7 @@ Definition deletionFinalizersForGarbageCollectionⁱᵐᵖˡ {ext : ffi_syntax} 
       else do:  #())));;;
     return: (#false, ![go.SliceType go.string] "oldFinalizers")).
 
-(* go: api_model.go:1240:6 *)
+(* go: api_model.go:1269:6 *)
 Definition newPreconditionUIDConflictErrorⁱᵐᵖˡ {ext : ffi_syntax} {go_gctx : GoGlobalContext} : val :=
   λ: "kind" "name" "preconditionUID" "uid",
     exception_do (let: "uid" := (GoAlloc go.string "uid") in
@@ -2485,7 +2578,7 @@ Definition newPreconditionUIDConflictErrorⁱᵐᵖˡ {ext : ffi_syntax} {go_gct
      (FuncResolve fmt.Errorf [] #()) "$a0" "$a1") in
      (FuncResolve errors.NewConflict [] #()) "$a0" "$a1" "$a2"))).
 
-(* go: api_model.go:1248:6 *)
+(* go: api_model.go:1277:6 *)
 Definition newUpdateUIDConflictErrorⁱᵐᵖˡ {ext : ffi_syntax} {go_gctx : GoGlobalContext} : val :=
   λ: "kind" "name" "existingUID" "uid",
     exception_do (let: "uid" := (GoAlloc types.UID "uid") in
@@ -2502,7 +2595,7 @@ Definition newUpdateUIDConflictErrorⁱᵐᵖˡ {ext : ffi_syntax} {go_gctx : Go
      (FuncResolve fmt.Errorf [] #()) "$a0" "$a1") in
      (FuncResolve errors.NewConflict [] #()) "$a0" "$a1" "$a2"))).
 
-(* go: api_model.go:1256:6 *)
+(* go: api_model.go:1285:6 *)
 Definition newUpdateResourceVersionConflictErrorⁱᵐᵖˡ {ext : ffi_syntax} {go_gctx : GoGlobalContext} : val :=
   λ: "kind" "name" "existingResourceVersion" "resourceVersion",
     exception_do (let: "resourceVersion" := (GoAlloc go.string "resourceVersion") in
@@ -2519,7 +2612,7 @@ Definition newUpdateResourceVersionConflictErrorⁱᵐᵖˡ {ext : ffi_syntax} {
      (FuncResolve fmt.Errorf [] #()) "$a0" "$a1") in
      (FuncResolve errors.NewConflict [] #()) "$a0" "$a1" "$a2"))).
 
-(* go: api_model.go:1264:6 *)
+(* go: api_model.go:1293:6 *)
 Definition newPreconditionRVConflictErrorⁱᵐᵖˡ {ext : ffi_syntax} {go_gctx : GoGlobalContext} : val :=
   λ: "kind" "name" "preconditionRV" "rv",
     exception_do (let: "rv" := (GoAlloc go.string "rv") in
@@ -2539,7 +2632,7 @@ Definition newPreconditionRVConflictErrorⁱᵐᵖˡ {ext : ffi_syntax} {go_gctx
 (* validateDeleteOptions checks structural DeleteOptions validation that upstream performs in BeforeDelete.
    Reference: https://github.com/kubernetes/kubernetes/blob/release-1.34/staging/src/k8s.io/apiserver/pkg/registry/rest/delete.go#L80-L81
 
-   go: api_model.go:1274:6 *)
+   go: api_model.go:1303:6 *)
 Definition validateDeleteOptionsⁱᵐᵖˡ {ext : ffi_syntax} {go_gctx : GoGlobalContext} : val :=
   λ: "options",
     exception_do (let: "options" := (GoAlloc (go.PointerType apis_meta_v1.DeleteOptions) "options") in
@@ -2563,7 +2656,7 @@ Definition validateDeleteOptionsⁱᵐᵖˡ {ext : ffi_syntax} {go_gctx : GoGlob
    Returns a Conflict error if preconditions don't match.
    Reference: https://github.com/kubernetes/kubernetes/blob/release-1.34/staging/src/k8s.io/apiserver/pkg/registry/rest/delete.go (BeforeDelete)
 
-   go: api_model.go:1288:6 *)
+   go: api_model.go:1317:6 *)
 Definition validateDeletePreconditionsⁱᵐᵖˡ {ext : ffi_syntax} {go_gctx : GoGlobalContext} : val :=
   λ: "metadata" "options" "kind",
     exception_do (let: "kind" := (GoAlloc go.string "kind") in
@@ -2600,7 +2693,7 @@ Definition validateDeletePreconditionsⁱᵐᵖˡ {ext : ffi_syntax} {go_gctx : 
    Returns (graceful, pendingGraceful, error).
    Reference: https://github.com/kubernetes/kubernetes/blob/release-1.34/pkg/registry/core/pod/strategy.go#L162-L191
 
-   go: api_model.go:1315:6 *)
+   go: api_model.go:1344:6 *)
 Definition checkGracefulDeleteⁱᵐᵖˡ {ext : ffi_syntax} {go_gctx : GoGlobalContext} : val :=
   λ: "obj" "options",
     exception_do (let: "options" := (GoAlloc (go.PointerType apis_meta_v1.DeleteOptions) "options") in
@@ -2767,7 +2860,7 @@ Definition checkGracefulDeleteⁱᵐᵖˡ {ext : ffi_syntax} {go_gctx : GoGlobal
    selfLink differences. This can still diverge from upstream in edge cases where storage
    normalization or Go representation details affect equality.
 
-   go: api_model.go:1424:6 *)
+   go: api_model.go:1453:6 *)
 Definition storageObjectDeepEqualⁱᵐᵖˡ {ext : ffi_syntax} {go_gctx : GoGlobalContext} : val :=
   λ: "obj1" "obj2",
     exception_do (let: "obj2" := (GoAlloc (go.InterfaceType []) "obj2") in
@@ -2806,7 +2899,7 @@ Definition storageObjectDeepEqualⁱᵐᵖˡ {ext : ffi_syntax} {go_gctx : GoGlo
      let: "$a1" := (![go.InterfaceType []] "obj2Copy") in
      (FuncResolve reflect.DeepEqual [] #()) "$a0" "$a1")).
 
-(* go: api_model.go:1440:6 *)
+(* go: api_model.go:1469:6 *)
 Definition shouldDeleteDuringUpdateⁱᵐᵖˡ {ext : ffi_syntax} {go_gctx : GoGlobalContext} : val :=
   λ: "objCopy" "existingObjCopy",
     exception_do (let: "existingObjCopy" := (GoAlloc (go.InterfaceType []) "existingObjCopy") in
@@ -2823,7 +2916,7 @@ Definition shouldDeleteDuringUpdateⁱᵐᵖˡ {ext : ffi_syntax} {go_gctx : GoG
    Reference: https://github.com/kubernetes/kubernetes/blob/release-1.34/staging/src/k8s.io/apiserver/pkg/registry/rest/delete.go#L163-L165
    Reference: https://github.com/kubernetes/kubernetes/blob/release-1.34/staging/src/k8s.io/apiserver/pkg/registry/generic/registry/store.go#L1022-L1028
 
-   go: api_model.go:1449:6 *)
+   go: api_model.go:1478:6 *)
 Definition deletionTimestampForDeleteⁱᵐᵖˡ {ext : ffi_syntax} {go_gctx : GoGlobalContext} : val :=
   λ: "graceful" "gracePeriod",
     exception_do (let: "gracePeriod" := (GoAlloc go.int64 "gracePeriod") in
@@ -2842,7 +2935,7 @@ Definition deletionTimestampForDeleteⁱᵐᵖˡ {ext : ffi_syntax} {go_gctx : G
     do:  ("now" <-[apis_meta_v1.Time] "$r0");;;
     return: ("now")).
 
-(* go: api_model.go:1461:17 *)
+(* go: api_model.go:1490:17 *)
 Definition State__deleteⁱᵐᵖˡ {ext : ffi_syntax} {go_gctx : GoGlobalContext} : val :=
   λ: "s" "key" "options",
     with_defer: (let: "s" := (GoAlloc (go.PointerType State) "s") in
@@ -2985,7 +3078,7 @@ Definition State__deleteⁱᵐᵖˡ {ext : ffi_syntax} {go_gctx : GoGlobalContex
 
 (* Returned value must be treated as read-only.
 
-   go: api_model.go:1560:17 *)
+   go: api_model.go:1589:17 *)
 Definition State__PodGetⁱᵐᵖˡ {ext : ffi_syntax} {go_gctx : GoGlobalContext} : val :=
   λ: "s" "namespace" "name",
     exception_do (let: "s" := (GoAlloc (go.PointerType State) "s") in
@@ -2996,7 +3089,7 @@ Definition State__PodGetⁱᵐᵖˡ {ext : ffi_syntax} {go_gctx : GoGlobalContex
     (MethodResolve (go.PointerType State) "PodMutGet"%go (![go.PointerType State] "s")) "$a0" "$a1")) in
     return: ("$ret0", "$ret1")).
 
-(* go: api_model.go:1564:17 *)
+(* go: api_model.go:1593:17 *)
 Definition State__PodMutGetⁱᵐᵖˡ {ext : ffi_syntax} {go_gctx : GoGlobalContext} : val :=
   λ: "s" "namespace" "name",
     exception_do (let: "s" := (GoAlloc (go.PointerType State) "s") in
@@ -3038,7 +3131,7 @@ Definition State__PodMutGetⁱᵐᵖˡ {ext : ffi_syntax} {go_gctx : GoGlobalCon
 
 (* Returned value must be treated as read-only.
 
-   go: api_model.go:1586:17 *)
+   go: api_model.go:1615:17 *)
 Definition State__PodListⁱᵐᵖˡ {ext : ffi_syntax} {go_gctx : GoGlobalContext} : val :=
   λ: "s" "namespace" "selector",
     exception_do (let: "s" := (GoAlloc (go.PointerType State) "s") in
@@ -3049,7 +3142,7 @@ Definition State__PodListⁱᵐᵖˡ {ext : ffi_syntax} {go_gctx : GoGlobalConte
     (MethodResolve (go.PointerType State) "PodMutList"%go (![go.PointerType State] "s")) "$a0" "$a1")) in
     return: ("$ret0", "$ret1")).
 
-(* go: api_model.go:1590:17 *)
+(* go: api_model.go:1619:17 *)
 Definition State__PodMutListⁱᵐᵖˡ {ext : ffi_syntax} {go_gctx : GoGlobalContext} : val :=
   λ: "s" "namespace" "selector",
     exception_do (let: "s" := (GoAlloc (go.PointerType State) "s") in
@@ -3097,7 +3190,7 @@ Definition State__PodMutListⁱᵐᵖˡ {ext : ffi_syntax} {go_gctx : GoGlobalCo
       do:  ("pods" <-[go.SliceType (go.PointerType api_core_v1.Pod)] "$r0")));;;
     return: (![go.SliceType (go.PointerType api_core_v1.Pod)] "pods", Convert go.untyped_nil go.error UntypedNil)).
 
-(* go: api_model.go:1608:17 *)
+(* go: api_model.go:1637:17 *)
 Definition State__PodCreateⁱᵐᵖˡ {ext : ffi_syntax} {go_gctx : GoGlobalContext} : val :=
   λ: "s" "namespace" "pod",
     exception_do (let: "s" := (GoAlloc (go.PointerType State) "s") in
@@ -3132,7 +3225,7 @@ Definition State__PodCreateⁱᵐᵖˡ {ext : ffi_syntax} {go_gctx : GoGlobalCon
     else do:  #());;;
     return: (![go.PointerType api_core_v1.Pod] "createdPod", Convert go.untyped_nil go.error UntypedNil)).
 
-(* go: api_model.go:1622:17 *)
+(* go: api_model.go:1651:17 *)
 Definition State__PodUpdateⁱᵐᵖˡ {ext : ffi_syntax} {go_gctx : GoGlobalContext} : val :=
   λ: "s" "namespace" "pod",
     exception_do (let: "s" := (GoAlloc (go.PointerType State) "s") in
@@ -3167,7 +3260,7 @@ Definition State__PodUpdateⁱᵐᵖˡ {ext : ffi_syntax} {go_gctx : GoGlobalCon
     else do:  #());;;
     return: (![go.PointerType api_core_v1.Pod] "updatedPod", Convert go.untyped_nil go.error UntypedNil)).
 
-(* go: api_model.go:1636:17 *)
+(* go: api_model.go:1665:17 *)
 Definition State__PodUpdateStatusⁱᵐᵖˡ {ext : ffi_syntax} {go_gctx : GoGlobalContext} : val :=
   λ: "s" "namespace" "pod",
     exception_do (let: "s" := (GoAlloc (go.PointerType State) "s") in
@@ -3202,7 +3295,7 @@ Definition State__PodUpdateStatusⁱᵐᵖˡ {ext : ffi_syntax} {go_gctx : GoGlo
     else do:  #());;;
     return: (![go.PointerType api_core_v1.Pod] "updatedPod", Convert go.untyped_nil go.error UntypedNil)).
 
-(* go: api_model.go:1650:17 *)
+(* go: api_model.go:1679:17 *)
 Definition State__PodDeleteⁱᵐᵖˡ {ext : ffi_syntax} {go_gctx : GoGlobalContext} : val :=
   λ: "s" "namespace" "name" "options",
     exception_do (let: "s" := (GoAlloc (go.PointerType State) "s") in
@@ -3221,7 +3314,7 @@ Definition State__PodDeleteⁱᵐᵖˡ {ext : ffi_syntax} {go_gctx : GoGlobalCon
 
 (* Returned value must be treated as read-only.
 
-   go: api_model.go:1661:17 *)
+   go: api_model.go:1690:17 *)
 Definition State__ReplicaSetGetⁱᵐᵖˡ {ext : ffi_syntax} {go_gctx : GoGlobalContext} : val :=
   λ: "s" "namespace" "name",
     exception_do (let: "s" := (GoAlloc (go.PointerType State) "s") in
@@ -3232,7 +3325,7 @@ Definition State__ReplicaSetGetⁱᵐᵖˡ {ext : ffi_syntax} {go_gctx : GoGloba
     (MethodResolve (go.PointerType State) "ReplicaSetMutGet"%go (![go.PointerType State] "s")) "$a0" "$a1")) in
     return: ("$ret0", "$ret1")).
 
-(* go: api_model.go:1665:17 *)
+(* go: api_model.go:1694:17 *)
 Definition State__ReplicaSetMutGetⁱᵐᵖˡ {ext : ffi_syntax} {go_gctx : GoGlobalContext} : val :=
   λ: "s" "namespace" "name",
     exception_do (let: "s" := (GoAlloc (go.PointerType State) "s") in
@@ -3274,7 +3367,7 @@ Definition State__ReplicaSetMutGetⁱᵐᵖˡ {ext : ffi_syntax} {go_gctx : GoGl
 
 (* Returned value must be treated as read-only.
 
-   go: api_model.go:1687:17 *)
+   go: api_model.go:1716:17 *)
 Definition State__ReplicaSetListⁱᵐᵖˡ {ext : ffi_syntax} {go_gctx : GoGlobalContext} : val :=
   λ: "s" "namespace" "selector",
     exception_do (let: "s" := (GoAlloc (go.PointerType State) "s") in
@@ -3285,7 +3378,7 @@ Definition State__ReplicaSetListⁱᵐᵖˡ {ext : ffi_syntax} {go_gctx : GoGlob
     (MethodResolve (go.PointerType State) "ReplicaSetMutList"%go (![go.PointerType State] "s")) "$a0" "$a1")) in
     return: ("$ret0", "$ret1")).
 
-(* go: api_model.go:1691:17 *)
+(* go: api_model.go:1720:17 *)
 Definition State__ReplicaSetMutListⁱᵐᵖˡ {ext : ffi_syntax} {go_gctx : GoGlobalContext} : val :=
   λ: "s" "namespace" "selector",
     exception_do (let: "s" := (GoAlloc (go.PointerType State) "s") in
@@ -3333,7 +3426,7 @@ Definition State__ReplicaSetMutListⁱᵐᵖˡ {ext : ffi_syntax} {go_gctx : GoG
       do:  ("rss" <-[go.SliceType (go.PointerType api_apps_v1.ReplicaSet)] "$r0")));;;
     return: (![go.SliceType (go.PointerType api_apps_v1.ReplicaSet)] "rss", Convert go.untyped_nil go.error UntypedNil)).
 
-(* go: api_model.go:1709:17 *)
+(* go: api_model.go:1738:17 *)
 Definition State__ReplicaSetCreateⁱᵐᵖˡ {ext : ffi_syntax} {go_gctx : GoGlobalContext} : val :=
   λ: "s" "namespace" "rs",
     exception_do (let: "s" := (GoAlloc (go.PointerType State) "s") in
@@ -3368,7 +3461,7 @@ Definition State__ReplicaSetCreateⁱᵐᵖˡ {ext : ffi_syntax} {go_gctx : GoGl
     else do:  #());;;
     return: (![go.PointerType api_apps_v1.ReplicaSet] "createdRS", Convert go.untyped_nil go.error UntypedNil)).
 
-(* go: api_model.go:1723:17 *)
+(* go: api_model.go:1752:17 *)
 Definition State__ReplicaSetUpdateⁱᵐᵖˡ {ext : ffi_syntax} {go_gctx : GoGlobalContext} : val :=
   λ: "s" "namespace" "rs",
     exception_do (let: "s" := (GoAlloc (go.PointerType State) "s") in
@@ -3403,7 +3496,7 @@ Definition State__ReplicaSetUpdateⁱᵐᵖˡ {ext : ffi_syntax} {go_gctx : GoGl
     else do:  #());;;
     return: (![go.PointerType api_apps_v1.ReplicaSet] "updatedRS", Convert go.untyped_nil go.error UntypedNil)).
 
-(* go: api_model.go:1737:17 *)
+(* go: api_model.go:1766:17 *)
 Definition State__ReplicaSetUpdateStatusⁱᵐᵖˡ {ext : ffi_syntax} {go_gctx : GoGlobalContext} : val :=
   λ: "s" "namespace" "rs",
     exception_do (let: "s" := (GoAlloc (go.PointerType State) "s") in
@@ -3438,7 +3531,7 @@ Definition State__ReplicaSetUpdateStatusⁱᵐᵖˡ {ext : ffi_syntax} {go_gctx 
     else do:  #());;;
     return: (![go.PointerType api_apps_v1.ReplicaSet] "updatedRS", Convert go.untyped_nil go.error UntypedNil)).
 
-(* go: api_model.go:1751:17 *)
+(* go: api_model.go:1780:17 *)
 Definition State__ReplicaSetDeleteⁱᵐᵖˡ {ext : ffi_syntax} {go_gctx : GoGlobalContext} : val :=
   λ: "s" "namespace" "name" "options",
     exception_do (let: "s" := (GoAlloc (go.PointerType State) "s") in
@@ -3457,7 +3550,7 @@ Definition State__ReplicaSetDeleteⁱᵐᵖˡ {ext : ffi_syntax} {go_gctx : GoGl
 
 (* Returned value must be treated as read-only.
 
-   go: api_model.go:1757:17 *)
+   go: api_model.go:1786:17 *)
 Definition State__PersistentVolumeClaimGetⁱᵐᵖˡ {ext : ffi_syntax} {go_gctx : GoGlobalContext} : val :=
   λ: "s" "namespace" "name",
     exception_do (let: "s" := (GoAlloc (go.PointerType State) "s") in
@@ -3468,7 +3561,7 @@ Definition State__PersistentVolumeClaimGetⁱᵐᵖˡ {ext : ffi_syntax} {go_gct
     (MethodResolve (go.PointerType State) "PersistentVolumeClaimMutGet"%go (![go.PointerType State] "s")) "$a0" "$a1")) in
     return: ("$ret0", "$ret1")).
 
-(* go: api_model.go:1761:17 *)
+(* go: api_model.go:1790:17 *)
 Definition State__PersistentVolumeClaimMutGetⁱᵐᵖˡ {ext : ffi_syntax} {go_gctx : GoGlobalContext} : val :=
   λ: "s" "namespace" "name",
     exception_do (let: "s" := (GoAlloc (go.PointerType State) "s") in
@@ -3510,7 +3603,7 @@ Definition State__PersistentVolumeClaimMutGetⁱᵐᵖˡ {ext : ffi_syntax} {go_
 
 (* Returned value must be treated as read-only.
 
-   go: api_model.go:1783:17 *)
+   go: api_model.go:1812:17 *)
 Definition State__PersistentVolumeClaimListⁱᵐᵖˡ {ext : ffi_syntax} {go_gctx : GoGlobalContext} : val :=
   λ: "s" "namespace" "selector",
     exception_do (let: "s" := (GoAlloc (go.PointerType State) "s") in
@@ -3521,7 +3614,7 @@ Definition State__PersistentVolumeClaimListⁱᵐᵖˡ {ext : ffi_syntax} {go_gc
     (MethodResolve (go.PointerType State) "PersistentVolumeClaimMutList"%go (![go.PointerType State] "s")) "$a0" "$a1")) in
     return: ("$ret0", "$ret1")).
 
-(* go: api_model.go:1787:17 *)
+(* go: api_model.go:1816:17 *)
 Definition State__PersistentVolumeClaimMutListⁱᵐᵖˡ {ext : ffi_syntax} {go_gctx : GoGlobalContext} : val :=
   λ: "s" "namespace" "selector",
     exception_do (let: "s" := (GoAlloc (go.PointerType State) "s") in
@@ -3569,7 +3662,7 @@ Definition State__PersistentVolumeClaimMutListⁱᵐᵖˡ {ext : ffi_syntax} {go
       do:  ("claims" <-[go.SliceType (go.PointerType api_core_v1.PersistentVolumeClaim)] "$r0")));;;
     return: (![go.SliceType (go.PointerType api_core_v1.PersistentVolumeClaim)] "claims", Convert go.untyped_nil go.error UntypedNil)).
 
-(* go: api_model.go:1805:17 *)
+(* go: api_model.go:1834:17 *)
 Definition State__PersistentVolumeClaimCreateⁱᵐᵖˡ {ext : ffi_syntax} {go_gctx : GoGlobalContext} : val :=
   λ: "s" "namespace" "pvc",
     exception_do (let: "s" := (GoAlloc (go.PointerType State) "s") in
@@ -3604,7 +3697,7 @@ Definition State__PersistentVolumeClaimCreateⁱᵐᵖˡ {ext : ffi_syntax} {go_
     else do:  #());;;
     return: (![go.PointerType api_core_v1.PersistentVolumeClaim] "createdPVC", Convert go.untyped_nil go.error UntypedNil)).
 
-(* go: api_model.go:1819:17 *)
+(* go: api_model.go:1848:17 *)
 Definition State__PersistentVolumeClaimUpdateⁱᵐᵖˡ {ext : ffi_syntax} {go_gctx : GoGlobalContext} : val :=
   λ: "s" "namespace" "pvc",
     exception_do (let: "s" := (GoAlloc (go.PointerType State) "s") in
@@ -3639,7 +3732,7 @@ Definition State__PersistentVolumeClaimUpdateⁱᵐᵖˡ {ext : ffi_syntax} {go_
     else do:  #());;;
     return: (![go.PointerType api_core_v1.PersistentVolumeClaim] "updatedPVC", Convert go.untyped_nil go.error UntypedNil)).
 
-(* go: api_model.go:1833:17 *)
+(* go: api_model.go:1862:17 *)
 Definition State__PersistentVolumeClaimUpdateStatusⁱᵐᵖˡ {ext : ffi_syntax} {go_gctx : GoGlobalContext} : val :=
   λ: "s" "namespace" "pvc",
     exception_do (let: "s" := (GoAlloc (go.PointerType State) "s") in
@@ -3674,7 +3767,7 @@ Definition State__PersistentVolumeClaimUpdateStatusⁱᵐᵖˡ {ext : ffi_syntax
     else do:  #());;;
     return: (![go.PointerType api_core_v1.PersistentVolumeClaim] "updatedPVC", Convert go.untyped_nil go.error UntypedNil)).
 
-(* go: api_model.go:1847:17 *)
+(* go: api_model.go:1876:17 *)
 Definition State__PersistentVolumeClaimDeleteⁱᵐᵖˡ {ext : ffi_syntax} {go_gctx : GoGlobalContext} : val :=
   λ: "s" "namespace" "name" "options",
     exception_do (let: "s" := (GoAlloc (go.PointerType State) "s") in
@@ -3693,7 +3786,7 @@ Definition State__PersistentVolumeClaimDeleteⁱᵐᵖˡ {ext : ffi_syntax} {go_
 
 (* Returned value must be treated as read-only.
 
-   go: api_model.go:1853:17 *)
+   go: api_model.go:1882:17 *)
 Definition State__StatefulSetGetⁱᵐᵖˡ {ext : ffi_syntax} {go_gctx : GoGlobalContext} : val :=
   λ: "s" "namespace" "name",
     exception_do (let: "s" := (GoAlloc (go.PointerType State) "s") in
@@ -3704,7 +3797,7 @@ Definition State__StatefulSetGetⁱᵐᵖˡ {ext : ffi_syntax} {go_gctx : GoGlob
     (MethodResolve (go.PointerType State) "StatefulSetMutGet"%go (![go.PointerType State] "s")) "$a0" "$a1")) in
     return: ("$ret0", "$ret1")).
 
-(* go: api_model.go:1857:17 *)
+(* go: api_model.go:1886:17 *)
 Definition State__StatefulSetMutGetⁱᵐᵖˡ {ext : ffi_syntax} {go_gctx : GoGlobalContext} : val :=
   λ: "s" "namespace" "name",
     exception_do (let: "s" := (GoAlloc (go.PointerType State) "s") in
@@ -3746,7 +3839,7 @@ Definition State__StatefulSetMutGetⁱᵐᵖˡ {ext : ffi_syntax} {go_gctx : GoG
 
 (* Returned value must be treated as read-only.
 
-   go: api_model.go:1879:17 *)
+   go: api_model.go:1908:17 *)
 Definition State__StatefulSetListⁱᵐᵖˡ {ext : ffi_syntax} {go_gctx : GoGlobalContext} : val :=
   λ: "s" "namespace" "selector",
     exception_do (let: "s" := (GoAlloc (go.PointerType State) "s") in
@@ -3757,7 +3850,7 @@ Definition State__StatefulSetListⁱᵐᵖˡ {ext : ffi_syntax} {go_gctx : GoGlo
     (MethodResolve (go.PointerType State) "StatefulSetMutList"%go (![go.PointerType State] "s")) "$a0" "$a1")) in
     return: ("$ret0", "$ret1")).
 
-(* go: api_model.go:1883:17 *)
+(* go: api_model.go:1912:17 *)
 Definition State__StatefulSetMutListⁱᵐᵖˡ {ext : ffi_syntax} {go_gctx : GoGlobalContext} : val :=
   λ: "s" "namespace" "selector",
     exception_do (let: "s" := (GoAlloc (go.PointerType State) "s") in
@@ -3805,7 +3898,7 @@ Definition State__StatefulSetMutListⁱᵐᵖˡ {ext : ffi_syntax} {go_gctx : Go
       do:  ("sets" <-[go.SliceType (go.PointerType api_apps_v1.StatefulSet)] "$r0")));;;
     return: (![go.SliceType (go.PointerType api_apps_v1.StatefulSet)] "sets", Convert go.untyped_nil go.error UntypedNil)).
 
-(* go: api_model.go:1901:17 *)
+(* go: api_model.go:1930:17 *)
 Definition State__StatefulSetCreateⁱᵐᵖˡ {ext : ffi_syntax} {go_gctx : GoGlobalContext} : val :=
   λ: "s" "namespace" "ss",
     exception_do (let: "s" := (GoAlloc (go.PointerType State) "s") in
@@ -3840,7 +3933,7 @@ Definition State__StatefulSetCreateⁱᵐᵖˡ {ext : ffi_syntax} {go_gctx : GoG
     else do:  #());;;
     return: (![go.PointerType api_apps_v1.StatefulSet] "createdSS", Convert go.untyped_nil go.error UntypedNil)).
 
-(* go: api_model.go:1915:17 *)
+(* go: api_model.go:1944:17 *)
 Definition State__StatefulSetUpdateⁱᵐᵖˡ {ext : ffi_syntax} {go_gctx : GoGlobalContext} : val :=
   λ: "s" "namespace" "ss",
     exception_do (let: "s" := (GoAlloc (go.PointerType State) "s") in
@@ -3875,7 +3968,7 @@ Definition State__StatefulSetUpdateⁱᵐᵖˡ {ext : ffi_syntax} {go_gctx : GoG
     else do:  #());;;
     return: (![go.PointerType api_apps_v1.StatefulSet] "updatedSS", Convert go.untyped_nil go.error UntypedNil)).
 
-(* go: api_model.go:1929:17 *)
+(* go: api_model.go:1958:17 *)
 Definition State__StatefulSetUpdateStatusⁱᵐᵖˡ {ext : ffi_syntax} {go_gctx : GoGlobalContext} : val :=
   λ: "s" "namespace" "ss",
     exception_do (let: "s" := (GoAlloc (go.PointerType State) "s") in
@@ -3910,7 +4003,7 @@ Definition State__StatefulSetUpdateStatusⁱᵐᵖˡ {ext : ffi_syntax} {go_gctx
     else do:  #());;;
     return: (![go.PointerType api_apps_v1.StatefulSet] "updatedSS", Convert go.untyped_nil go.error UntypedNil)).
 
-(* go: api_model.go:1943:17 *)
+(* go: api_model.go:1972:17 *)
 Definition State__StatefulSetDeleteⁱᵐᵖˡ {ext : ffi_syntax} {go_gctx : GoGlobalContext} : val :=
   λ: "s" "namespace" "name" "options",
     exception_do (let: "s" := (GoAlloc (go.PointerType State) "s") in
@@ -3929,7 +4022,7 @@ Definition State__StatefulSetDeleteⁱᵐᵖˡ {ext : ffi_syntax} {go_gctx : GoG
 
 (* Returned value must be treated as read-only.
 
-   go: api_model.go:1949:17 *)
+   go: api_model.go:1978:17 *)
 Definition State__DeploymentGetⁱᵐᵖˡ {ext : ffi_syntax} {go_gctx : GoGlobalContext} : val :=
   λ: "s" "namespace" "name",
     exception_do (let: "s" := (GoAlloc (go.PointerType State) "s") in
@@ -3940,7 +4033,7 @@ Definition State__DeploymentGetⁱᵐᵖˡ {ext : ffi_syntax} {go_gctx : GoGloba
     (MethodResolve (go.PointerType State) "DeploymentMutGet"%go (![go.PointerType State] "s")) "$a0" "$a1")) in
     return: ("$ret0", "$ret1")).
 
-(* go: api_model.go:1953:17 *)
+(* go: api_model.go:1982:17 *)
 Definition State__DeploymentMutGetⁱᵐᵖˡ {ext : ffi_syntax} {go_gctx : GoGlobalContext} : val :=
   λ: "s" "namespace" "name",
     exception_do (let: "s" := (GoAlloc (go.PointerType State) "s") in
@@ -3986,7 +4079,7 @@ Definition State__DeploymentMutGetⁱᵐᵖˡ {ext : ffi_syntax} {go_gctx : GoGl
 
 (* Returned value must be treated as read-only.
 
-   go: api_model.go:1975:17 *)
+   go: api_model.go:2004:17 *)
 Definition State__DeploymentListⁱᵐᵖˡ {ext : ffi_syntax} {go_gctx : GoGlobalContext} : val :=
   λ: "s" "namespace" "selector",
     exception_do (let: "s" := (GoAlloc (go.PointerType State) "s") in
@@ -3997,7 +4090,7 @@ Definition State__DeploymentListⁱᵐᵖˡ {ext : ffi_syntax} {go_gctx : GoGlob
     (MethodResolve (go.PointerType State) "DeploymentMutList"%go (![go.PointerType State] "s")) "$a0" "$a1")) in
     return: ("$ret0", "$ret1")).
 
-(* go: api_model.go:1979:17 *)
+(* go: api_model.go:2008:17 *)
 Definition State__DeploymentMutListⁱᵐᵖˡ {ext : ffi_syntax} {go_gctx : GoGlobalContext} : val :=
   λ: "s" "namespace" "selector",
     exception_do (let: "s" := (GoAlloc (go.PointerType State) "s") in
@@ -4045,7 +4138,7 @@ Definition State__DeploymentMutListⁱᵐᵖˡ {ext : ffi_syntax} {go_gctx : GoG
       do:  ("deployments" <-[go.SliceType (go.PointerType api_apps_v1.Deployment)] "$r0")));;;
     return: (![go.SliceType (go.PointerType api_apps_v1.Deployment)] "deployments", Convert go.untyped_nil go.error UntypedNil)).
 
-(* go: api_model.go:1997:17 *)
+(* go: api_model.go:2026:17 *)
 Definition State__DeploymentCreateⁱᵐᵖˡ {ext : ffi_syntax} {go_gctx : GoGlobalContext} : val :=
   λ: "s" "namespace" "d",
     exception_do (let: "s" := (GoAlloc (go.PointerType State) "s") in
@@ -4080,7 +4173,7 @@ Definition State__DeploymentCreateⁱᵐᵖˡ {ext : ffi_syntax} {go_gctx : GoGl
     else do:  #());;;
     return: (![go.PointerType api_apps_v1.Deployment] "createdDeployment", Convert go.untyped_nil go.error UntypedNil)).
 
-(* go: api_model.go:2011:17 *)
+(* go: api_model.go:2040:17 *)
 Definition State__DeploymentUpdateⁱᵐᵖˡ {ext : ffi_syntax} {go_gctx : GoGlobalContext} : val :=
   λ: "s" "namespace" "d",
     exception_do (let: "s" := (GoAlloc (go.PointerType State) "s") in
@@ -4115,7 +4208,7 @@ Definition State__DeploymentUpdateⁱᵐᵖˡ {ext : ffi_syntax} {go_gctx : GoGl
     else do:  #());;;
     return: (![go.PointerType api_apps_v1.Deployment] "updatedDeployment", Convert go.untyped_nil go.error UntypedNil)).
 
-(* go: api_model.go:2025:17 *)
+(* go: api_model.go:2054:17 *)
 Definition State__DeploymentUpdateStatusⁱᵐᵖˡ {ext : ffi_syntax} {go_gctx : GoGlobalContext} : val :=
   λ: "s" "namespace" "d",
     exception_do (let: "s" := (GoAlloc (go.PointerType State) "s") in
@@ -4150,7 +4243,7 @@ Definition State__DeploymentUpdateStatusⁱᵐᵖˡ {ext : ffi_syntax} {go_gctx 
     else do:  #());;;
     return: (![go.PointerType api_apps_v1.Deployment] "updatedDeployment", Convert go.untyped_nil go.error UntypedNil)).
 
-(* go: api_model.go:2039:17 *)
+(* go: api_model.go:2068:17 *)
 Definition State__DeploymentDeleteⁱᵐᵖˡ {ext : ffi_syntax} {go_gctx : GoGlobalContext} : val :=
   λ: "s" "namespace" "name" "options",
     exception_do (let: "s" := (GoAlloc (go.PointerType State) "s") in
@@ -4166,6 +4259,122 @@ Definition State__DeploymentDeleteⁱᵐᵖˡ {ext : ffi_syntax} {go_gctx : GoGl
     return: (let: "$a0" := (![KKey] "key") in
      let: "$a1" := (![apis_meta_v1.DeleteOptions] "options") in
      (MethodResolve (go.PointerType State) "delete"%go (![go.PointerType State] "s")) "$a0" "$a1")).
+
+(* Returned value must be treated as read-only.
+
+   go: api_model.go:2074:17 *)
+Definition State__NamespaceGetⁱᵐᵖˡ {ext : ffi_syntax} {go_gctx : GoGlobalContext} : val :=
+  λ: "s" "name",
+    exception_do (let: "s" := (GoAlloc (go.PointerType State) "s") in
+    let: "name" := (GoAlloc go.string "name") in
+    let: "key" := (GoAlloc KKey (GoZeroVal KKey #())) in
+    let: "$r0" := (let: "$v0" := #"Namespace"%go in
+    let: "$v1" := (![go.string] "name") in
+    CompositeLiteral KKey (LiteralValue [KeyedElement (Some (KeyField "Kind"%go)) (ElementExpression go.string "$v0"); KeyedElement (Some (KeyField "Name"%go)) (ElementExpression go.string "$v1")])) in
+    do:  ("key" <-[KKey] "$r0");;;
+    let: "err" := (GoAlloc go.error (GoZeroVal go.error #())) in
+    let: "obj" := (GoAlloc (go.InterfaceType []) (GoZeroVal (go.InterfaceType []) #())) in
+    let: ("$ret0", "$ret1") := (let: "$a0" := (![KKey] "key") in
+    (MethodResolve (go.PointerType State) "get"%go (![go.PointerType State] "s")) "$a0") in
+    let: "$r0" := "$ret0" in
+    let: "$r1" := "$ret1" in
+    do:  ("obj" <-[go.InterfaceType []] "$r0");;;
+    do:  ("err" <-[go.error] "$r1");;;
+    (if: Convert go.untyped_bool go.bool ((![go.error] "err") ≠⟨go.error⟩ (Convert go.untyped_nil go.error UntypedNil))
+    then return: (Convert go.untyped_nil (go.PointerType api_core_v1.Namespace) UntypedNil, ![go.error] "err")
+    else do:  #());;;
+    let: "ok" := (GoAlloc go.bool (GoZeroVal go.bool #())) in
+    let: "namespace" := (GoAlloc (go.PointerType api_core_v1.Namespace) (GoZeroVal (go.PointerType api_core_v1.Namespace) #())) in
+    let: ("$ret0", "$ret1") := (TypeAssert2 (go.PointerType api_core_v1.Namespace) (![go.InterfaceType []] "obj")) in
+    let: "$r0" := "$ret0" in
+    let: "$r1" := "$ret1" in
+    do:  ("namespace" <-[go.PointerType api_core_v1.Namespace] "$r0");;;
+    do:  ("ok" <-[go.bool] "$r1");;;
+    (if: (⟨go.bool⟩! (![go.bool] "ok"))
+    then
+      return: (Convert go.untyped_nil (go.PointerType api_core_v1.Namespace) UntypedNil, let: "$a0" := #"state entry for namespace %s is not a *v1.Namespace"%go in
+       let: "$a1" := ((let: "$sl0" := (Convert go.string go.any (![go.string] "name")) in
+       CompositeLiteral (go.SliceType go.any) (LiteralValue [KeyedElement None (ElementExpression go.any "$sl0")]))) in
+       (FuncResolve fmt.Errorf [] #()) "$a0" "$a1")
+    else do:  #());;;
+    return: (![go.PointerType api_core_v1.Namespace] "namespace", Convert go.untyped_nil go.error UntypedNil)).
+
+(* Returned value must be treated as read-only.
+
+   go: api_model.go:2092:17 *)
+Definition State__ServiceAccountGetⁱᵐᵖˡ {ext : ffi_syntax} {go_gctx : GoGlobalContext} : val :=
+  λ: "s" "namespace" "name",
+    exception_do (let: "s" := (GoAlloc (go.PointerType State) "s") in
+    let: "name" := (GoAlloc go.string "name") in
+    let: "namespace" := (GoAlloc go.string "namespace") in
+    let: "key" := (GoAlloc KKey (GoZeroVal KKey #())) in
+    let: "$r0" := (let: "$v0" := #"ServiceAccount"%go in
+    let: "$v1" := (![go.string] "namespace") in
+    let: "$v2" := (![go.string] "name") in
+    CompositeLiteral KKey (LiteralValue [KeyedElement (Some (KeyField "Kind"%go)) (ElementExpression go.string "$v0"); KeyedElement (Some (KeyField "Namespace"%go)) (ElementExpression go.string "$v1"); KeyedElement (Some (KeyField "Name"%go)) (ElementExpression go.string "$v2")])) in
+    do:  ("key" <-[KKey] "$r0");;;
+    let: "err" := (GoAlloc go.error (GoZeroVal go.error #())) in
+    let: "obj" := (GoAlloc (go.InterfaceType []) (GoZeroVal (go.InterfaceType []) #())) in
+    let: ("$ret0", "$ret1") := (let: "$a0" := (![KKey] "key") in
+    (MethodResolve (go.PointerType State) "get"%go (![go.PointerType State] "s")) "$a0") in
+    let: "$r0" := "$ret0" in
+    let: "$r1" := "$ret1" in
+    do:  ("obj" <-[go.InterfaceType []] "$r0");;;
+    do:  ("err" <-[go.error] "$r1");;;
+    (if: Convert go.untyped_bool go.bool ((![go.error] "err") ≠⟨go.error⟩ (Convert go.untyped_nil go.error UntypedNil))
+    then return: (Convert go.untyped_nil (go.PointerType api_core_v1.ServiceAccount) UntypedNil, ![go.error] "err")
+    else do:  #());;;
+    let: "ok" := (GoAlloc go.bool (GoZeroVal go.bool #())) in
+    let: "serviceAccount" := (GoAlloc (go.PointerType api_core_v1.ServiceAccount) (GoZeroVal (go.PointerType api_core_v1.ServiceAccount) #())) in
+    let: ("$ret0", "$ret1") := (TypeAssert2 (go.PointerType api_core_v1.ServiceAccount) (![go.InterfaceType []] "obj")) in
+    let: "$r0" := "$ret0" in
+    let: "$r1" := "$ret1" in
+    do:  ("serviceAccount" <-[go.PointerType api_core_v1.ServiceAccount] "$r0");;;
+    do:  ("ok" <-[go.bool] "$r1");;;
+    (if: (⟨go.bool⟩! (![go.bool] "ok"))
+    then
+      return: (Convert go.untyped_nil (go.PointerType api_core_v1.ServiceAccount) UntypedNil, let: "$a0" := #"state entry for serviceaccount %s/%s is not a *v1.ServiceAccount"%go in
+       let: "$a1" := ((let: "$sl0" := (Convert go.string go.any (![go.string] "namespace")) in
+       let: "$sl1" := (Convert go.string go.any (![go.string] "name")) in
+       CompositeLiteral (go.SliceType go.any) (LiteralValue [KeyedElement None (ElementExpression go.any "$sl0"); KeyedElement None (ElementExpression go.any "$sl1")]))) in
+       (FuncResolve fmt.Errorf [] #()) "$a0" "$a1")
+    else do:  #());;;
+    return: (![go.PointerType api_core_v1.ServiceAccount] "serviceAccount", Convert go.untyped_nil go.error UntypedNil)).
+
+(* go: api_model.go:2113:17 *)
+Definition State__ServiceAccountCreateⁱᵐᵖˡ {ext : ffi_syntax} {go_gctx : GoGlobalContext} : val :=
+  λ: "s" "namespace" "serviceAccount",
+    exception_do (let: "s" := (GoAlloc (go.PointerType State) "s") in
+    let: "serviceAccount" := (GoAlloc (go.PointerType api_core_v1.ServiceAccount) "serviceAccount") in
+    let: "namespace" := (GoAlloc go.string "namespace") in
+    let: "err" := (GoAlloc go.error (GoZeroVal go.error #())) in
+    let: "obj" := (GoAlloc (go.InterfaceType []) (GoZeroVal (go.InterfaceType []) #())) in
+    let: ("$ret0", "$ret1") := (let: "$a0" := #"ServiceAccount"%go in
+    let: "$a1" := (![go.string] "namespace") in
+    let: "$a2" := (Convert (go.PointerType api_core_v1.ServiceAccount) (go.InterfaceType []) (![go.PointerType api_core_v1.ServiceAccount] "serviceAccount")) in
+    (MethodResolve (go.PointerType State) "create"%go (![go.PointerType State] "s")) "$a0" "$a1" "$a2") in
+    let: "$r0" := "$ret0" in
+    let: "$r1" := "$ret1" in
+    do:  ("obj" <-[go.InterfaceType []] "$r0");;;
+    do:  ("err" <-[go.error] "$r1");;;
+    (if: Convert go.untyped_bool go.bool ((![go.error] "err") ≠⟨go.error⟩ (Convert go.untyped_nil go.error UntypedNil))
+    then return: (Convert go.untyped_nil (go.PointerType api_core_v1.ServiceAccount) UntypedNil, ![go.error] "err")
+    else do:  #());;;
+    let: "ok" := (GoAlloc go.bool (GoZeroVal go.bool #())) in
+    let: "createdServiceAccount" := (GoAlloc (go.PointerType api_core_v1.ServiceAccount) (GoZeroVal (go.PointerType api_core_v1.ServiceAccount) #())) in
+    let: ("$ret0", "$ret1") := (TypeAssert2 (go.PointerType api_core_v1.ServiceAccount) (![go.InterfaceType []] "obj")) in
+    let: "$r0" := "$ret0" in
+    let: "$r1" := "$ret1" in
+    do:  ("createdServiceAccount" <-[go.PointerType api_core_v1.ServiceAccount] "$r0");;;
+    do:  ("ok" <-[go.bool] "$r1");;;
+    (if: (⟨go.bool⟩! (![go.bool] "ok"))
+    then
+      return: (Convert go.untyped_nil (go.PointerType api_core_v1.ServiceAccount) UntypedNil, let: "$a0" := #"create returned unexpected type %T"%go in
+       let: "$a1" := ((let: "$sl0" := (![go.InterfaceType []] "obj") in
+       CompositeLiteral (go.SliceType go.any) (LiteralValue [KeyedElement None (ElementExpression go.any "$sl0")]))) in
+       (FuncResolve fmt.Errorf [] #()) "$a0" "$a1")
+    else do:  #());;;
+    return: (![go.PointerType api_core_v1.ServiceAccount] "createdServiceAccount", Convert go.untyped_nil go.error UntypedNil)).
 
 (* go: transaction.go:13:6 *)
 Definition preconditionUIDMismatchⁱᵐᵖˡ {ext : ffi_syntax} {go_gctx : GoGlobalContext} : val :=
@@ -4470,7 +4679,7 @@ Definition State__updateStatusTxⁱᵐᵖˡ {ext : ffi_syntax} {go_gctx : GoGlob
 
 #[global] Instance info' : PkgInfo pkg_id.apimodel :=
 {|
-  pkg_imported_pkgs := [code.context.pkg_id.context; code.fmt.pkg_id.fmt; code.math.rand.pkg_id.rand; code.reflect.pkg_id.reflect; code.strconv.pkg_id.strconv; code.sync.pkg_id.sync; code.time.pkg_id.time; code.k8s_io.api.apps.v1.pkg_id.v1; code.k8s_io.api.core.v1.pkg_id.v1; code.k8s_io.apimachinery.pkg.api.errors.pkg_id.errors; code.k8s_io.apimachinery.pkg.api.meta.pkg_id.meta; code.k8s_io.apimachinery.pkg.api.validation.pkg_id.validation; code.k8s_io.apimachinery.pkg.apis.meta.v1.pkg_id.v1; code.k8s_io.apimachinery.pkg.apis.meta.v1.validation.pkg_id.validation; code.k8s_io.apimachinery.pkg.labels.pkg_id.labels; code.k8s_io.apimachinery.pkg.runtime.pkg_id.runtime; code.k8s_io.apimachinery.pkg.runtime.schema.pkg_id.schema; code.k8s_io.apimachinery.pkg.types.pkg_id.types; code.k8s_io.apimachinery.pkg.util.uuid.pkg_id.uuid; code.k8s_io.apimachinery.pkg.util.validation.field.pkg_id.field; code.k8s_io.apiserver.pkg.endpoints.request.pkg_id.request; code.k8s_io.apiserver.pkg.registry.generic.registry.pkg_id.registry; code.k8s_io.apiserver.pkg.registry.rest.pkg_id.rest; code.k8s_io.kubernetes.pkg.api.legacyscheme.pkg_id.legacyscheme; code.k8s_io.kubernetes.pkg.apis.apps.pkg_id.apps; code.k8s_io.kubernetes.pkg.apis.apps.v1.pkg_id.v1; code.k8s_io.kubernetes.pkg.apis.core.pkg_id.core; code.k8s_io.kubernetes.pkg.apis.core.v1.pkg_id.v1; code.k8s_io.kubernetes.pkg.controller.pkg_id.controller; code.k8s_io.kubernetes.pkg.registry.apps.deployment.pkg_id.deployment; code.k8s_io.kubernetes.pkg.registry.apps.replicaset.pkg_id.replicaset; code.k8s_io.kubernetes.pkg.registry.apps.statefulset.pkg_id.statefulset; code.k8s_io.kubernetes.pkg.registry.core.persistentvolumeclaim.pkg_id.persistentvolumeclaim; code.k8s_io.kubernetes.pkg.registry.core.pod.pkg_id.pod; code.k8s_io.kubernetes.pkg.apis.apps.install.pkg_id.install]
+  pkg_imported_pkgs := [code.context.pkg_id.context; code.fmt.pkg_id.fmt; code.math.rand.pkg_id.rand; code.reflect.pkg_id.reflect; code.strconv.pkg_id.strconv; code.sync.pkg_id.sync; code.time.pkg_id.time; code.k8s_io.api.apps.v1.pkg_id.v1; code.k8s_io.api.core.v1.pkg_id.v1; code.k8s_io.apimachinery.pkg.api.errors.pkg_id.errors; code.k8s_io.apimachinery.pkg.api.meta.pkg_id.meta; code.k8s_io.apimachinery.pkg.api.validation.pkg_id.validation; code.k8s_io.apimachinery.pkg.apis.meta.v1.pkg_id.v1; code.k8s_io.apimachinery.pkg.apis.meta.v1.validation.pkg_id.validation; code.k8s_io.apimachinery.pkg.labels.pkg_id.labels; code.k8s_io.apimachinery.pkg.runtime.pkg_id.runtime; code.k8s_io.apimachinery.pkg.runtime.schema.pkg_id.schema; code.k8s_io.apimachinery.pkg.types.pkg_id.types; code.k8s_io.apimachinery.pkg.util.uuid.pkg_id.uuid; code.k8s_io.apimachinery.pkg.util.validation.field.pkg_id.field; code.k8s_io.apiserver.pkg.endpoints.request.pkg_id.request; code.k8s_io.apiserver.pkg.registry.generic.registry.pkg_id.registry; code.k8s_io.apiserver.pkg.registry.rest.pkg_id.rest; code.k8s_io.kubernetes.pkg.api.legacyscheme.pkg_id.legacyscheme; code.k8s_io.kubernetes.pkg.apis.apps.pkg_id.apps; code.k8s_io.kubernetes.pkg.apis.apps.v1.pkg_id.v1; code.k8s_io.kubernetes.pkg.apis.core.pkg_id.core; code.k8s_io.kubernetes.pkg.apis.core.v1.pkg_id.v1; code.k8s_io.kubernetes.pkg.controller.pkg_id.controller; code.k8s_io.kubernetes.pkg.registry.apps.deployment.pkg_id.deployment; code.k8s_io.kubernetes.pkg.registry.apps.replicaset.pkg_id.replicaset; code.k8s_io.kubernetes.pkg.registry.apps.statefulset.pkg_id.statefulset; code.k8s_io.kubernetes.pkg.registry.core.persistentvolumeclaim.pkg_id.persistentvolumeclaim; code.k8s_io.kubernetes.pkg.registry.core.pod.pkg_id.pod; code.k8s_io.kubernetes.pkg.registry.core.serviceaccount.pkg_id.serviceaccount; code.k8s_io.kubernetes.pkg.apis.apps.install.pkg_id.install]
 |}.
 
 Definition initialize' {ext : ffi_syntax} {go_gctx : GoGlobalContext} : val :=
@@ -4478,6 +4687,7 @@ Definition initialize' {ext : ffi_syntax} {go_gctx : GoGlobalContext} : val :=
     package.init pkg_id.apimodel (λ: <>,
       exception_do (do:  (go.GlobalAlloc ModelState (go.PointerType State) #());;;
       do:  (install.initialize' #());;;
+      do:  (serviceaccount.initialize' #());;;
       do:  (pod.initialize' #());;;
       do:  (persistentvolumeclaim.initialize' #());;;
       do:  (statefulset.initialize' #());;;
@@ -4575,6 +4785,7 @@ Class State_Assumptions {ext : ffi_syntax} `{!GoGlobalContext} `{!GoLocalContext
   #[global] State'ptr_DeploymentUpdate_unfold :: MethodUnfold (go.PointerType (State)) "DeploymentUpdate" (State__DeploymentUpdateⁱᵐᵖˡ);
   #[global] State'ptr_DeploymentUpdateStatus_unfold :: MethodUnfold (go.PointerType (State)) "DeploymentUpdateStatus" (State__DeploymentUpdateStatusⁱᵐᵖˡ);
   #[global] State'ptr_Index_unfold :: MethodUnfold (go.PointerType (State)) "Index" (State__Indexⁱᵐᵖˡ);
+  #[global] State'ptr_NamespaceGet_unfold :: MethodUnfold (go.PointerType (State)) "NamespaceGet" (State__NamespaceGetⁱᵐᵖˡ);
   #[global] State'ptr_PersistentVolumeClaimCreate_unfold :: MethodUnfold (go.PointerType (State)) "PersistentVolumeClaimCreate" (State__PersistentVolumeClaimCreateⁱᵐᵖˡ);
   #[global] State'ptr_PersistentVolumeClaimDelete_unfold :: MethodUnfold (go.PointerType (State)) "PersistentVolumeClaimDelete" (State__PersistentVolumeClaimDeleteⁱᵐᵖˡ);
   #[global] State'ptr_PersistentVolumeClaimGet_unfold :: MethodUnfold (go.PointerType (State)) "PersistentVolumeClaimGet" (State__PersistentVolumeClaimGetⁱᵐᵖˡ);
@@ -4600,6 +4811,8 @@ Class State_Assumptions {ext : ffi_syntax} `{!GoGlobalContext} `{!GoLocalContext
   #[global] State'ptr_ReplicaSetMutList_unfold :: MethodUnfold (go.PointerType (State)) "ReplicaSetMutList" (State__ReplicaSetMutListⁱᵐᵖˡ);
   #[global] State'ptr_ReplicaSetUpdate_unfold :: MethodUnfold (go.PointerType (State)) "ReplicaSetUpdate" (State__ReplicaSetUpdateⁱᵐᵖˡ);
   #[global] State'ptr_ReplicaSetUpdateStatus_unfold :: MethodUnfold (go.PointerType (State)) "ReplicaSetUpdateStatus" (State__ReplicaSetUpdateStatusⁱᵐᵖˡ);
+  #[global] State'ptr_ServiceAccountCreate_unfold :: MethodUnfold (go.PointerType (State)) "ServiceAccountCreate" (State__ServiceAccountCreateⁱᵐᵖˡ);
+  #[global] State'ptr_ServiceAccountGet_unfold :: MethodUnfold (go.PointerType (State)) "ServiceAccountGet" (State__ServiceAccountGetⁱᵐᵖˡ);
   #[global] State'ptr_StatefulSetCreate_unfold :: MethodUnfold (go.PointerType (State)) "StatefulSetCreate" (State__StatefulSetCreateⁱᵐᵖˡ);
   #[global] State'ptr_StatefulSetDelete_unfold :: MethodUnfold (go.PointerType (State)) "StatefulSetDelete" (State__StatefulSetDeleteⁱᵐᵖˡ);
   #[global] State'ptr_StatefulSetGet_unfold :: MethodUnfold (go.PointerType (State)) "StatefulSetGet" (State__StatefulSetGetⁱᵐᵖˡ);
@@ -4743,6 +4956,7 @@ Class Assumptions {ext : ffi_syntax} `{!GoGlobalContext} `{!GoLocalContext} `{!G
   #[global] import_statefulset_Assumption :: statefulset.Assumptions;
   #[global] import_persistentvolumeclaim_Assumption :: persistentvolumeclaim.Assumptions;
   #[global] import_pod_Assumption :: pod.Assumptions;
+  #[global] import_serviceaccount_Assumption :: serviceaccount.Assumptions;
   #[global] import_install_Assumption :: install.Assumptions;
 }.
 End apimodel.
